Splitting MGProofs into multiple parts (PropMarked subdirectory) and continuing work on proofs

Click/MGProofs.v
@@ -15,6 +15,11 @@ Require Import Click.Definitions.
 Require Import Click.Invariants.
 Require Import Click.MG.
 
+Require Import Click.PropMarked.PropMarked.
+Require Import Click.PropMarked.Step.
+Require Import Click.PropMarked.Outgoing.
+Require Import Click.PropMarked.StepPreserved.
+
 Require Import Omega.
 
 
@@ -24,18 +29,16 @@ Require Import Coq.Program.Equality.
 Require Import Coq.Logic.FunctionalExtensionality.
 
 
-Module ClickMGProofs (ClickModule : ClickType).
+Module ClickMGProofs (Export PropMarked : PropMarkedType).
 
-  Module ClickMG := ClickMG(ClickModule).
-  Import ClickMG.
-  Import ClickTactics.
+  Export PropMarked.ClickMG.
+  Export ClickTactics.
 
+  Module Import PropMarkedTactics := PropMarkedTactics PropMarked.
+  Module Import StepImpliesPropMarked := StepImpliesPropMarked PropMarked.
+  Module Import OutgoingPlaceNotMarked := OutgoingPlaceNotMarked PropMarked.
+  Module Import StepPreservation := StepPreservation PropMarked.
 
-  Definition latch_in_flag (l : latch even odd) := swap_token_flag (latch_to_token_flag l).
-  Definition latch_out_flag (l : latch even odd) := latch_to_token_flag l.
-  Definition latch_stage_MG l := stage_MG (latch_in_flag l) (latch_out_flag l).
-  Definition latch_transition_event l := transition_event l (latch_in_flag l).
-  Definition latch_stage_MG_SS l := stage_MG_SS l (latch_in_flag l).
 
   (* The theorem *)
   Theorem MG_refines_stage : forall l,
@@ -218,127 +221,11 @@ Qed.
 
 
 
-
-
-  (************************** TODO ********************************)
-
-  (** Intuitively, [prop_marked p σ] is a property that holds on a state σ
-  whenever a related marking m satisfies [m(p) > 0]. *)
-  Section prop_marked.
-
-
-  Variable l : latch even odd.
-  Inductive prop_marked : forall {t1 t2} (p : stage_place t1 t2) (σ : state name), Prop :=
-
-  (* left_ack -> left_req *)
-  | lack_lreq_marked σ :
-    σ (ack (latch_input l)) = σ (req (latch_input l)) -> prop_marked left_ack_left_req σ
-
-  (* right_req -> right_ack *)
-  | rreq_rack_marked σ :
-    σ (req (latch_output l)) = neg_value (σ (ack (latch_output l))) ->
-    prop_marked right_req_right_ack σ (* right_req -> right_ack *)
-
-  (* clk- -> left_ack *)
-  | clk_fall_left_ack_marked σ :
-    σ (latch_clk l) = Bit0 ->
-(*    σ (latch_old_clk l) = Bit0 -> (* i.e. flop component is stable *) *)
-    (* The left_ack component is unstable *)
-    σ (ack (latch_input l)) = match latch_to_token_flag l with
-                              | Token => σ (latch_state0 l)
-                              | Nontoken => neg_value (σ (latch_state0 l))
-                              end ->
-(*    σ (req (latch_input l)) = σ (ack (latch_input l)) -> (* left environment is stable *)*)
-    prop_marked clk_fall_left_ack σ
-
-  | clk_fall_left_ack_state0_marked σ :
-    σ (latch_clk l) = Bit0 ->
-    σ (latch_old_clk l) = Bit1 ->
-    prop_marked clk_fall_left_ack σ
-
-  (* clk+ -> right_req *)
-  | clk_rise_right_req_marked σ :
-    σ (latch_clk l) = Bit1 ->
-    σ (latch_old_clk l) = Bit0 ->
-    prop_marked clk_rise_right_req σ
-  | clk_rise_right_req_marked_state0 σ :
-    σ (req (latch_output l)) <> σ (latch_state0 l) ->
-(*    σ (ack (latch_output l)) <> σ (req (latch_output l)) -> *)
-    prop_marked clk_rise_right_req σ
-
-  (* clk+ -> clk- *)
-  | clock_fall_flop_marked σ :
-    σ (latch_clk l) = Bit1 ->
-    σ (latch_old_clk l) = Bit0 ->
-    stable (latch_clk_component l) σ ->
-    prop_marked clock_fall σ
-  | clock_fall_state0_marked σ :
-    σ (latch_clk l) = Bit1 ->
-    σ (latch_old_clk l) = Bit1 ->
-    ~ stable (latch_clk_component l) σ ->
-    prop_marked clock_fall σ
-
-  (* left_req -> clk+ *)
-  | left_req_clk_rise_marked σ :
-    σ (req (latch_input l)) = neg_value (σ (ack (latch_input l))) ->
-    latch_clk_function l σ = Bit1 ->
-    σ (latch_clk l) = Bit0 ->
-    prop_marked left_req_clk_rise σ
-
-  (* right_ack -> clk+ *)
-  | right_ack_clk_rise_marked σ :
-    σ (ack (latch_output l)) = σ (req (latch_output l)) ->
-    latch_clk_function l σ = Bit1 ->
-    σ (latch_clk l) = Bit0 ->
-    prop_marked right_ack_clk_rise σ
-  .
-
-Import ClickTactics.
-
-
-  Lemma init_relate_implies_marked : forall {t1 t2} (p : stage_place t1 t2),
-    prop_marked p (σR l) ->
-    init_marking (latch_stage_MG l) _ _ p > 0.
-  Proof.
-    intros t1 t2 p Hp.
-    dependent destruction Hp;
-      try (simpl; unfold init_marking_flag; simpl;
-      unfold σR in *; simpl in *; reduce_eqb;
-      try (destruct l; simpl in *; find_contradiction; auto; fail);
-    fail).
-  Qed.
-
-Lemma wf_reset_hidden_1 : forall σ,
-    wf_stage_state l σ ->
-    σ match latch_to_token_flag l with
-      | Token => dp_reset_n
-      | NonToken => latch_hidden l
-      end = Bit1.
-Proof.
-  intros ? Hwf.
-  destruct l.
-    apply wf_hidden; auto.
-    eapply wf_dp_reset_n; eauto.
-Qed.
-Lemma wf_hidden_reset_1 : forall σ,
-    wf_stage_state l σ ->
-    σ match latch_to_token_flag l with
-      | Token => latch_hidden l
-      | NonToken => dp_reset_n
-      end = Bit1.
-Proof.
-  intros ? Hwf.
-  destruct l.
-    eapply wf_dp_reset_n; eauto.
-    apply wf_hidden; auto.
-Qed.
-Hint Resolve wf_reset_hidden_1 wf_hidden_reset_1 : wf.
-
-Lemma latch_clk_function_is_bit : forall σ,
+Lemma latch_clk_function_is_bit : forall l σ,
     wf_stage_state l σ ->
     val_is_bit (latch_clk_function l σ).
 Proof.
-  intros σ Hwf.
+  intros l σ Hwf.
   assert (Hlreq : val_is_bit (σ (req (latch_input l)))) by solve_val_is_bit.
   assert (Hstate0 : val_is_bit (σ (latch_state0 l))) by solve_val_is_bit.
   assert (Hrack :  val_is_bit (σ (ack (latch_output l)))) by solve_val_is_bit.
@@ -362,1205 +249,11 @@ Qed.
 Hint Resolve latch_clk_function_is_bit : wf.
 
 
-  Section step_implies_prop_marked.
-
-    Variable σ σ' : state name.
-    Hypothesis Hwf : wf_stage_state l σ.
-(*    Hypothesis Hwf_stable : wf_stage_state_stable l σ. *)
-
-
-
-  Definition step_implies_prop_marked_spec {t t0} (p : stage_place t0 t) :=
-    latch_stage_with_env l ⊢ σ →{Some (latch_transition_event l t σ)} Some σ' ->
-    prop_marked p σ.
-
-  Lemma step_implies_prop_marked_left_ack_left_req :
-    step_implies_prop_marked_spec left_ack_left_req.
-  Proof.
-    intros Hstep.
-      constructor.
-      unfold latch_transition_event, transition_event in Hstep.
-      step_inversion_clean.
-      combine_state_equiv_on_domain.
-
-      apply val_is_bit_neg_inversion in Heq.
-      2:{ solve_val_is_bit. }
-      simpl.
-      rewrite <- Heq.
-      apply val_is_bit_neg_inversion.
-      { solve_val_is_bit. }
-      reflexivity.
-  Unshelve. exact (fun _ => true).
-  Qed.
-
-  Lemma step_implies_prop_marked_clk_fall_left_ack :
-    step_implies_prop_marked_spec clk_fall_left_ack.
-  Proof.
-    intros Hstep. 
-      unfold latch_transition_event, transition_event in Hstep.
-
-      step_inversion_clean.
-      clear Hin0.
-      combine_state_equiv_on_complex.
-      { simpl. solve_space_set. }
-      combine_state_equiv_on_domain.
-
-      simpl in Hguard. destruct Hguard as [Hclk Hstate0].
-
-      apply clk_fall_left_ack_marked; auto.
-        apply val_is_bit_neq in Hunstable; try solve_val_is_bit.
-        simpl. rewrite <- Hunstable.
-        destruct l; simpl; auto.
-        rewrite val_is_bit_neg_neg; try solve_val_is_bit; auto.
-  Unshelve. exact (fun _ => true).
-  Qed.
-
-  Lemma step_implies_prop_marked_clk_rise_right_req :
-    step_implies_prop_marked_spec clk_rise_right_req.
-  Proof.
-    intros Hstep.
-      replace (latch_transition_event l right_req σ)
-        with  (Event (req (latch_output l)) (neg_value (σ (req (latch_output l)))))
-        in    Hstep
-        by    auto.
-      step_inversion_clean.
-      clear Hin0.
-      combine_state_equiv_on_domain.
-      destruct Hin as [Hin | Hin].
-      2:{ contradict Hin. unfold update. reduce_eqb.
-          apply bit_neq_neg_r; try solve_val_is_bit.
-      }
-      apply clk_rise_right_req_marked_state0.
-      { apply val_is_bit_neq_neg; auto.
-        { right; solve_val_is_bit. }
-      }
-    Unshelve. exact (fun _ => true).
-  Qed. 
-
-  Lemma step_implies_prop_marked_right_req_right_ack :
-    step_implies_prop_marked_spec right_req_right_ack.
-  Proof.
-    intros Hstep.
-      constructor.
-      unfold latch_transition_event, transition_event in Hstep.
-      step_inversion_clean.
-  Unshelve. exact (fun _ => true).
-  Qed.
-
-
-  Lemma step_implies_prop_marked_clock_fall :
-    step_implies_prop_marked_spec clock_fall.
-  Proof.
-    intros Hstep.
-    replace (latch_transition_event l clk_fall σ)
-      with  (Event (latch_clk l) Bit0)
-      in    Hstep
-      by    auto.
-    step_inversion_clean.
-    clear Hin. clear Hdec.
-    combine_state_equiv_on_complex. { simpl; solve_space_set. }
-    
-    apply flop_inversion_clk in Hstep3.
-    2:{ solve_all_disjoint. }
-    2:{ auto with wf. }
-    2:{ auto with wf. }
-    destruct Hstep3 as [Hequiv' Hstep3].
-    combine_state_equiv_on.
-    standardize_state_equiv_on_set Hequiv0.
-    combine_state_equiv_on_domain.
-
-    assert (Hclk : σ (latch_clk l) = Bit1).
-    { rewrite <- Heq in *.
-      apply val_is_bit_neq in Hunstable; try solve_val_is_bit.
-    }
-
-    apply clock_fall_state0_marked; auto.
-    { (* old_clk *) rewrite <- Hstep3; auto. }
-    Print latch_clk_component.
-    Search stable func_space.
-    intros Hstable; apply func_stable_equiv in Hstable.
-    2:{ solve_space_set. }
-    contradict Hstable; auto.
-
-  Unshelve.
-    exact (fun _ => true).
-  Qed.
-
-  Lemma step_implies_prop_marked_left_req_clk_rise :
-    step_implies_prop_marked_spec left_req_clk_rise.
-  Proof.
-    intros Hstep.
-    replace (latch_transition_event l clk_rise σ)
-      with  (Event (latch_clk l) Bit1)
-      in    Hstep
-      by    auto.
-
-    step_inversion_clean.
-    clear Hin.
-    combine_state_equiv_on_complex. { simpl; solve_space_set. }
-    
-    apply flop_inversion_clk in Hstep3.
-    2:{ solve_all_disjoint. }
-    2:{ auto with wf. }
-    2:{ auto with wf. }
-
-    destruct Hstep3 as [Hequiv' Hstep3].
-    combine_state_equiv_on.
-    combine_state_equiv_on_domain.
-
-    apply left_req_clk_rise_marked; auto.
-    { (* Uses latch_clk_function_Bit1_l_req and wf_left_env *)
-      compare (σ (req (latch_input l)))
-              (σ (ack (latch_input l))).
-      2:{ symmetry. apply val_is_bit_neq; try solve_val_is_bit. }
-      symmetry in Heq0.
-      assert (Hreq : σ (req (latch_input l)) <> if_token l (σ (latch_state0 l))).
-      { rewrite <- Heq0. 
-        apply wf_left_env in Heq0; auto.
-        rewrite Heq0.
-        apply not_eq_sym.
-        destruct l; apply bit_neq_neg_r; simpl; solve_val_is_bit.
-      }
-      contradict Hreq.
-      apply latch_clk_function_Bit1_l_req; auto.
-    }
-    { apply val_is_bit_neq in Hunstable;
-        try solve_val_is_bit; auto with wf.
-        simpl. rewrite <- Hunstable.
-        rewrite <- Heq. auto.
-    }
-
-    Unshelve. exact (fun _ => true).
-
-  Qed.
-
-  Lemma step_implies_prop_marked_right_ack_clk_rise :
-    step_implies_prop_marked_spec right_ack_clk_rise.
-  Proof.
-    intros Hstep.
-    replace (latch_transition_event l clk_rise σ)
-      with  (Event (latch_clk l) Bit1)
-      in    Hstep
-      by    auto.
-    step_inversion_clean.
-    clear Hin. clear Hdec.
-    combine_state_equiv_on_complex.
-    { simpl; solve_space_set. }
-
-    apply flop_inversion_clk in Hstep3.
-    2:{ solve_all_disjoint. }
-    2:{ auto with wf. }
-    2:{ auto with wf. }
-
-    destruct Hstep3 as [Hequiv' Hstep3].
-
-    combine_state_equiv_on.
-    combine_state_equiv_on_domain.
-
-    apply right_ack_clk_rise_marked; auto.
-    { (* Uses latch_clk_function_Bit1_r_ack and wf_right_env *)
-      compare (σ (req (latch_output l)))
-              (σ (ack (latch_output l))); auto.
-      assert (Hneq1 : σ (req (latch_output l)) = neg_value (σ (ack (latch_output l)))).
-      { symmetry; apply  val_is_bit_neq; try solve_val_is_bit. }
-      assert (Hneq2 : σ (ack (latch_output l)) = neg_value (σ (req (latch_output l)))).
-      { symmetry; apply  val_is_bit_neq; try solve_val_is_bit. }
-      clear Hneq.
-      assert (Hack : σ (ack (latch_output l)) = σ (latch_state0 l)).
-      { apply latch_clk_function_Bit1_r_ack; auto. }
-      apply wf_right_env in Hneq2; auto.
-      contradict Hneq1.
-      { rewrite Hneq2. rewrite Hack.
-        apply bit_neq_neg_r; solve_val_is_bit.
-      }
-    }
-    { rewrite Hstep3.
-      apply val_is_bit_neq in Hunstable; try solve_val_is_bit; auto with wf.
-      rewrite <- Hstep3. simpl.
-      rewrite <- Hunstable.
-      rewrite <- Heq.
-      auto.
-    }
-
-
-    Unshelve. exact (fun _ => true).
-  Qed.
-
-
-  End step_implies_prop_marked.
-
-  Lemma step_implies_prop_marked : forall σ t σ',
-    wf_stage_state l σ ->
-    latch_stage_with_env l ⊢ σ →{Some (latch_transition_event l t σ)} Some σ' ->
-    forall t0 (p : stage_place t0 t), prop_marked p σ.
-  Proof.
-    intros σ t σ' Hwf Hstep t0 p.
-    dependent destruction p.
-    { eapply step_implies_prop_marked_left_ack_left_req; eauto. }
-    { eapply step_implies_prop_marked_clk_fall_left_ack; eauto. }
-    { eapply step_implies_prop_marked_clk_rise_right_req; eauto. }
-    { eapply step_implies_prop_marked_right_req_right_ack; eauto. }
-    { eapply step_implies_prop_marked_clock_fall; eauto. }
-    { eapply step_implies_prop_marked_left_req_clk_rise; eauto. }
-    { eapply step_implies_prop_marked_right_ack_clk_rise; eauto. }
-  Qed.
-
-  Lemma stage_eps_decide_state0 : forall σ σ0,
-    wf_stage_state l σ ->
-
-    latch_stage_with_env l ⊢ σ →{None} Some σ0 ->
-    σ (latch_state0 l) <> σ0 (latch_state0 l) ->
-    σ (latch_old_clk l) = Bit1 \/ σ (latch_clk l) = Bit1.
-  Proof.
-    intros σ σ' Hwf Hstep Hstate0.
-    apply step_implies_stage_eps in Hstep; auto.
-    inversion Hstep as [ Hclk Hold_clk Hequiv
-                       | v Hclk Hold_clk Hv Hclk_function Hl_ack Hr_req Hnot_state0 Hequiv
-                       | Hnot_state0 Hclk Hequiv
-                       ]; subst; clear Hstep.
-
-    * left.
-      apply val_is_bit_neq in Hold_clk; try solve_val_is_bit.
-      rewrite <- Hold_clk.
-      apply val_is_bit_neq in Hclk; try solve_val_is_bit.
-
-    * right; auto.
-
-    * contradict Hstate0.
-      rewrite_state_equiv. 2:{ solve_in_dom. }
-      simpl; auto.
-  Qed.
-
-
-  Arguments wf_scoped {name} S {S_wf} σ e σ' Hstep x : rename.
-
-Ltac rewrite_back_wf_scoped :=
-  match goal with
-  | [ Hstep : ?S ⊢ ?σ →{ ?e } Some ?σ' |- context[ ?σ ?x ] ] =>
-    erewrite <- (wf_scoped S σ e σ' Hstep x);
-    [ | try (intro; inversion 1; find_contradiction; fail)
-    | rewrite latch_stage_with_env_input, latch_stage_with_env_output;
-          solve_space_set
-    ]
-  end.
-
-
-
-  (* Helper lemmas for relate_implies_marked below *)
-  Lemma relate_implies_marked_eps : forall σ σ',
-    wf_stage_state l σ ->
-    latch_stage_with_env l ⊢ σ →{None} Some σ' ->
-    forall {t1 t2} (p : stage_place t1 t2),
-    prop_marked p σ' ->
-    prop_marked p σ.
-  Proof.
-    intros σ σ' Hwf Hstep t1 t2 p Hp.
-    dependent destruction Hp.
-    * (* left_ack_left_req *) 
-      (* Because σ0 left_ack = σ0 left_req, if σ →{None} σ0,
-         then it must be the case that σ is equivalent to σ0 on left_ack and left_req. *)
-      apply lack_lreq_marked.
-
-      rewrite_back_wf_scoped.
-      rewrite_back_wf_scoped.
-      auto.
-
-    * (* right_req_right_ack *)
-      apply rreq_rack_marked.
-      rewrite_back_wf_scoped.
-      rewrite_back_wf_scoped.
-      auto.
-
-    * (* clk_fall_left_ack *)
-      assert (Hclk : σ (latch_clk l) = Bit0).
-      { rewrite_back_wf_scoped; auto. }
-      assert (Hack : σ (ack (latch_input l)) = σ0 (ack (latch_input l))).
-      { rewrite_back_wf_scoped; auto. }
-
-      assert (Hstate0 : σ (latch_state0 l) = σ0 (latch_state0 l) -> prop_marked clk_fall_left_ack σ).
-      { intros Hstate0.
-        apply clk_fall_left_ack_marked; auto.
-        rewrite Hack. rewrite Hstate0. auto.
-      }
-      assert (Hold_clk : σ (latch_old_clk l) = Bit1 ->
-                        prop_marked clk_fall_left_ack σ).
-      { intros Hold_clk.
-        apply clk_fall_left_ack_state0_marked; auto.
-      }
-
-      compare (σ (latch_state0 l)) (σ0 (latch_state0 l)); auto.
-      apply stage_eps_decide_state0 in Hstep; auto.
-      destruct Hstep as [Hstep | Hstep]; auto.
-      { find_contradiction. }
-
-    * (* clk_fall_left_ack *)
-      assert (Hclk : σ (latch_clk l) = Bit0) by (rewrite_back_wf_scoped; auto).
-
-      apply clk_fall_left_ack_state0_marked; auto.
-      apply step_implies_stage_eps in Hstep; auto.
-      inversion Hstep; subst; find_contradiction; clear Hstep.
-      + apply val_is_bit_neq in H2; auto; try solve_val_is_bit.
-        rewrite <- H2. rewrite Hclk. auto.
-      + contradict H0.
-        rewrite <- H3. 2:{ solve_in_dom. }
-        unfold update.
-        rewrite <- H2. rewrite Hclk. simpl. inversion 1.
-
-
-    * assert (Hclk : σ (latch_clk l) = Bit1).
-      { rewrite_back_wf_scoped; auto. }
-      apply clk_rise_right_req_marked; auto.
-
-      apply step_implies_stage_eps in Hstep; auto.
-      inversion Hstep; subst; find_contradiction; clear Hstep.
-      + contradict H0. (* old_clk *)
-        rewrite_state_equiv.
-        2:{ solve_in_dom. }
-        reduce_eqb.
-        rewrite Hclk; inversion 1.
-
-      + contradict H0 (* old_clk *).
-        rewrite_state_equiv.
-        2:{ solve_in_dom. }
-        rewrite <- H2, Hclk. simpl. inversion 1.
-
-    * assert (Hclk : σ (req (latch_output l)) = σ0 (req (latch_output l))).
-      { rewrite_back_wf_scoped; auto. }
-
-      apply step_implies_stage_eps in Hstep; auto.
-      inversion Hstep; subst; find_contradiction; clear Hstep.
-      + apply clk_rise_right_req_marked_state0.
-        contradict H.
-        rewrite_state_equiv. 2:{ solve_in_dom. }
-        rewrite_state_equiv. 2:{ solve_in_dom. }
-        simpl. auto.
-
-      + (* If state0 is getting updated, so σ state0 <> σ0 state0... *)
-        apply clk_rise_right_req_marked; auto.
-        apply not_eq_sym in H1.
-        apply val_is_bit_neq in H1 (* old_clk *); try solve_val_is_bit.
-
-      + apply clk_rise_right_req_marked_state0.
-        contradict H.
-        rewrite_state_equiv. 2:{ solve_in_dom. }
-        rewrite_state_equiv. 2:{ solve_in_dom. }
-        simpl. auto.
-
-
-    * (* clk_fall *)
-
-      assert (Hclk : σ (latch_clk l) = Bit1).
-      { rewrite_back_wf_scoped; auto. }
-      assert (Hold_clk : σ (latch_old_clk l) = Bit0).
-      { (* In case 1: Bit0 = σ0 old_clk = σ clk = Bit1 
-           In case 2: Bit0 = σ0 old_clk = σ clk = Bit1
-           In case 3: Bit0 = σ0 old_clk = σ old_clk
-        *)
-        apply step_implies_stage_eps in Hstep; auto.
-        inversion Hstep; subst; find_contradiction; clear Hstep.
-        + apply not_eq_sym in H3. (* old_clk *)
-          apply val_is_bit_neq in H3 (* old_clk *); try solve_val_is_bit.
-        + contradict H0. rewrite_state_equiv.
-          2:{ rewrite dom_latch_stage_with_env; solve_space_set. }
-          rewrite <- H3, Hclk.
-          simpl. inversion 1.
-      }
-      assert (Hwf' : wf_stage_state l σ0).
-      { eapply step_wf_state_eps; eauto. }
-      assert (Hl_req : σ (req (latch_input l)) = σ0 (req (latch_input l)))
-        by (rewrite_back_wf_scoped; auto).
-      assert (Hr_ack : σ (ack (latch_output l)) = σ0 (ack (latch_output l)))
-        by (rewrite_back_wf_scoped; auto).
-
-      apply clock_fall_flop_marked; auto.
-      (*   In case 1: σ0 state0 = σ state0, so this follows.
-           In case 3: σ0 state0 = σ state0, so this follows.
-
-           In case 2: the clk component can go from stable to unstable by changing state0, but not unstable to stable... why must this be the case?
-
-           Lemma: if ⊢ σ →{None} Some σ'
-                  and latch_clk_function l σ' = Bit1
-                  then latch_clk_function l σ = Bit1
-        *)
-        apply func_stable_equiv. { solve_space_set. }
-        apply func_stable_equiv in H1. 2:{ solve_space_set. }
-
-        apply step_implies_stage_eps in Hstep; auto.
-        inversion Hstep; subst; find_contradiction; clear Hstep.
-        + auto.
-        + compare Bit1 (latch_clk_function l σ); auto.
-          { rewrite <- Heq; auto. }
-          (* when they are not equal *)
-          apply val_is_bit_neq in Hneq; try solve_val_is_bit; auto with wf.
-          simpl in Hneq.
-
-          (* If σ == σ0 on everything except latch_not_state0 *)
-
-          rewrite latch_clk_function_equiv with (σ' := σ0).
-          { rewrite Hclk.  rewrite <- H. auto. }
-          { prove_equiv_subset. }
-
-    * (* clock_fall *)
-      assert (Hclk : σ (latch_clk l) = Bit1)
-        by (rewrite_back_wf_scoped; auto).
-
-      apply step_implies_stage_eps in Hstep; auto.
-      inversion Hstep; subst; find_contradiction; clear Hstep.
-      + apply clock_fall_flop_marked; auto.
-        { (* old_clk *)
-          apply not_eq_sym in H3. (* old_clk *)
-          apply val_is_bit_neq in H3 (* latch_old_clk *); try solve_val_is_bit.
-        }
-        { (* stable *)
-          apply func_stable_equiv. { solve_space_set. }
-          auto.
-        }
-
-      + apply clock_fall_state0_marked; auto.
-        { (* old_clk *)
-          rewrite <- H3. auto.
-        }
-        { intros Hstable.
-          apply H1.
-          apply func_stable_equiv in Hstable.
-          2:{ solve_space_set. }
-          apply func_stable_equiv.
-          { solve_space_set. }
-          rewrite_state_equiv. 2:{ solve_in_dom. }
-          simpl.
-          rewrite latch_clk_function_equiv with (σ' := σ).
-          2:{ intros x Hx. rewrite <- H4 (* state_equiv_on *).
-              2:{ decompose_set_structure; solve_in_dom. }
-              unfold update. compare_next; auto.
-              contradict Hx; solve_space_set.
-          }
-          auto.
-        }
-
-    * (* left_req_clk_rise *)
-      assert (Hclk : σ (latch_clk l) = σ0 (latch_clk l)).
-      { rewrite_back_wf_scoped; auto. }
-
-      apply left_req_clk_rise_marked; auto.
-      { rewrite_back_wf_scoped. rewrite_back_wf_scoped.
-        auto.
-      }
-      { rewrite latch_clk_function_equiv with (σ' := σ0); auto.
-        { apply step_implies_stage_eps in Hstep; auto.
-          inversion Hstep; subst; find_contradiction; clear Hstep.
-          + intros x Hx.
-            decompose_set_structure; rewrite_state_equiv; auto; solve_in_dom.
-
-          + contradict Hclk.
-            rewrite H1. (* σ0 clk = Bit0 *)
-            rewrite H2. (* σ clk = Bit1 *)
-            inversion 1.
-
-          + intros x Hx.
-            decompose_set_structure; rewrite_state_equiv; auto; solve_in_dom.
-        }
-      }
-      rewrite Hclk. auto.
-
-    * (* right_ack_clk_rise *)
-      assert (Hclk : σ (latch_clk l) = σ0 (latch_clk l)).
-      { rewrite_back_wf_scoped; auto. }
-
-      apply right_ack_clk_rise_marked.
-      { rewrite_back_wf_scoped. rewrite_back_wf_scoped. auto. }
-      { rewrite latch_clk_function_equiv with (σ' := σ0); auto.
-        { apply step_implies_stage_eps in Hstep; auto.
-          inversion Hstep; subst; find_contradiction; clear Hstep.
-          + intros x Hx.
-            decompose_set_structure; rewrite_state_equiv; auto; solve_in_dom.
-
-          + contradict Hclk.
-            rewrite H1 (* σ0 clk = Bit0 *).
-            rewrite H2 (* σ clk = Bit1 *).
-            inversion 1.
-
-          + intros x Hx.
-            decompose_set_structure; rewrite_state_equiv; auto; solve_in_dom.
-        }
-      }
-      { rewrite Hclk. auto. }
-
-  Unshelve. all:auto.
-
-  Qed.
-
-
-
-  Lemma outgoing_place_not_marked : forall σ σ' t,
-    wf_stage_state l σ ->
-    latch_stage_with_env l ⊢ σ →{Some (latch_transition_event l t σ)} Some σ' ->
-    forall t0 (p : stage_place t0 t),
-        ~ prop_marked p σ'.
-  Proof.
-    intros σ σ' t Hwf Hstep t0 p Hprop.
-
-    dependent destruction Hprop.
-    * (* t = left_req *)
-      unfold latch_transition_event, transition_event in Hstep.
-
-      step_inversion_clean.
-      combine_state_equiv_on_domain.
-
-      apply neg_value_inj in Heq; try solve_val_is_bit.
-      (* Know:
-
-         H : σ left_ack = σ0 left_ack = σ0 left_req = neg_value (σ left_req)
-         Heq : σ left_req = σ left_ack
-      *)
-      contradict H.
-      repeat (rewrite_state_equiv; try solve_in_dom).
-      simpl. reduce_eqb.
-      rewrite Heq.
-      apply bit_neq_neg_r; try solve_val_is_bit.
-
-    * (* t = right_ack *)
-      unfold latch_transition_event, transition_event in Hstep.
-      step_inversion_clean.
-      combine_state_equiv_on_domain.
-
-      (* Know:
-         H : σ right_req = σ0 right_req  = neg_value (σ0 right_ack) = neg_value (neg_value (σ right_ack))
-         Heq : neg_value (σ right_ack) = σ right_req
-      *)
-      contradict H.
-      repeat (rewrite_state_equiv; try solve_in_dom).
-      simpl. reduce_eqb.
-      rewrite <- Heq.
-      apply bit_neq_neg_r; solve_val_is_bit.
-
-    * (* t = left_ack (1) *)
-      replace (latch_transition_event l left_ack σ)
-          with (Event (ack (latch_input l)) (neg_value (σ (ack (latch_input l)))))
-          in Hstep
-          by auto.
-      step_inversion_clean.
-      clear Hin0.
-      destruct Hguard as [Hclk Hstate0].
-      combine_state_equiv_on_complex; try (simpl; solve_space_set).
-      combine_state_equiv_on_domain.
-      (* Know:
-         H : σ clk = σ0 clk = Bit0
-         H0 : neg_value (σ l_ack) = σ0 l_ack = if_token l (σ0 state0) = if_token l (σ state0)
-         Heq : neg_value (σ l_ack) = if_token l (neg_value (σ state0))
-         Hunstable : if_token l (neg_value (σ state0)) <> σ l_ack
-         Hclk : σ clk = Bit0
-         Hstate0 : σ not_state0 = neg_value (σ state0)
-      *)
-      contradict H0.
-      repeat (rewrite_state_equiv; try solve_in_dom).
-      simpl. reduce_eqb.
-      rewrite Heq.
-      destruct l; simpl; [ | apply not_eq_sym ]; apply bit_neq_neg_r; simpl;
-        try solve_val_is_bit.
-
-
-   * (* t = left_ack (2) *)
-
-     replace (latch_transition_event l left_ack σ)
-          with (Event (ack (latch_input l)) (neg_value (σ (ack (latch_input l)))))
-          in Hstep
-          by auto.
-     step_inversion_clean.
-     clear Hin0.
-     combine_state_equiv_on_complex; try (simpl; solve_space_set).
-     combine_state_equiv_on_domain.
-     destruct Hguard as [Hclk Hstate0].
-     (* Know:
-        H0 : Heq : neg_value l_ack = if_token l (neg_value (σ state0))
-        Hunstable : if_token l (neg_value (σ state0)) <> σ l_ack
-        Hstate0 : σ not_state0 = neg_value (σ state0)
-     *)
-     assert (H_ack_stable : ~ stable (latch_left_ack_component l) σ).
-     { intros [_ Hstable]. (* if it were, then it would not have taken a step *)
-       assert (Hstep' : latch_left_ack_component l ⊢ σ 
-                →{Some (Event (ack (latch_input l)) (neg_value (σ (ack (latch_input l)))))}
-                Some σ0).
-        { apply delay_space_output.
-          3:{ solve_space_set. }
-          3:{ intros x Hx. rewrite_state_equiv; try solve_in_dom.
-              compare_next; auto.
-              decompose_set_structure.
-          }
-          { split; auto. }
-          apply func_output.
-          { simpl. rewrite <- Heq.
-            apply bit_neq_neg_r; try solve_val_is_bit.
-          }
-          { simpl. rewrite <- Heq; auto. }
-          { intros x Hx. rewrite_state_equiv; try solve_in_dom.
-            auto.
-          }
-        }
-        specialize (Hstable _ _ Hstep').
-        inversion Hstable as [? Hstable']; subst.
-        contradict Hstable'.
-        simpl. solve_space_set.
-    }
-
-
-    set (flop_set := match latch_to_token_flag l with
-                     | Token => dp_reset_n
-                     | NonToken => latch_hidden l
-                     end).
-    set (flop_reset := match latch_to_token_flag l with
-                       | NonToken => dp_reset_n
-                       | Token => latch_hidden l
-                     end).
-    assert (H_flop_stable : ~ stable (flop flop_set flop_reset
-                                           (latch_clk l) (latch_old_clk l)
-                                           (latch_not_state0 l) (latch_state0 l))
-                                     σ).
-    { intros Hstable.
-      Print flop_step.
-      assert (Hstep : flop flop_set flop_reset
-                           (latch_clk l) (latch_old_clk l)
-                           (latch_not_state0 l) (latch_state0 l)
-                      ⊢ σ →{None} Some (update σ (latch_old_clk l) (σ (latch_clk l)))).
-      { apply Flop_clk_fall; auto.
-        { rewrite Hclk; inversion 1. }
-        { rewrite Hclk.
-          replace (σ (latch_old_clk l)) with (σ0 (latch_old_clk l)).
-          2:{ rewrite_state_equiv; try solve_in_dom. auto. }
-          rewrite H0; inversion 1.
-        }
-        { intros x Hx. auto. }
-       }
-       destruct Hstable as [_ Hstable].
-       specialize (Hstable _ _ Hstep).
-       inversion Hstable.
-    }
-
-
-    (* Know:
-       H : σ clk = σ0 clk = Bit0
-       H0 : σ old_clk = σ0 old_clk = Bit1
-       Heq : neg_value (σ l_ack) = if_token l (neg_value (σ state0))
-         aka σ l_ack = if_token l (σ state0)
-       Hstate0 : σ not_state0 = neg_value (σ state0)
-
-       Heq+wf_left_env ==> σ l_ack <> σ l_req
-    *)
-    (* I think we need to modify the timing constraint/delay so that the clk-
-    event has time to propogate not just to clk, but also to the flop. Can we do
-    this by modifying flop so that clk- events update old_clk automatically??
-    *)
-    admit.
-
-  * (* t = right_req (1) *)
-    replace (latch_transition_event l right_req σ)
-          with (Event (req (latch_output l)) (neg_value (σ (req (latch_output l)))))
-          in Hstep
-          by auto.
-    step_inversion_clean.
-    combine_state_equiv_on_domain.
-    clear Hin0.
-    (* Know:
-       H : σ clk = σ0 clk = Bit1
-       H0 : σ old_clk = σ0 old_clk = Bit0
-       Heq : neg_value (σ r_req) = σ state0
-       Hunstable : σ state0 <> σ r_req
-    *)
-    (* Since the flop is unstable on clk+, it must be the case that
-         latch_clk_function σ = Bit1 [ BUT WHY?]
-       Therefore, it must be the case that 
-         σ (ack (latch_output l)) = σ (latch_state0 l)
-       from latch_clk_function_Bit1_r_ack.
-       But this means that
-         σ r_ack = neg_value (σ r_req)
-       By wf_right_env, this implies that
-         σ r_req = σ state0
-       which is a contradiction.
-    *)
-    assert (Hfun : latch_clk_function l σ = Bit1).
-    { (* Some invariant about the fact that σ clk = Bit1 and σ old_clk = Bit0.... *)
-      admit.
-    }
-    apply latch_clk_function_Bit1_r_ack in Hfun; auto.
-    assert (Hunstable' : σ (ack (latch_output l)) = neg_value (σ (req (latch_output l)))).
-    { rewrite Hfun. Search (neg_value _ = _).
-      symmetry in Heq. apply val_is_bit_neg_inversion in Heq; try solve_val_is_bit.
-      simpl. rewrite <- Heq.
-      rewrite val_is_bit_neg_neg; try solve_val_is_bit.
-    }
-    apply wf_right_env in Hunstable'; auto; find_contradiction.
-
-  * (* t = right_req (2) *)
-    replace (latch_transition_event l right_req σ)
-          with (Event (req (latch_output l)) (neg_value (σ (req (latch_output l)))))
-          in Hstep
-          by auto.
-    step_inversion_clean.
-    combine_state_equiv_on_domain.
-    clear Hin0.
-    (* Know:
-       H : neg_value (σ r_req) = σ0 r_req <> σ0 state0 = σ state0
-       aka    σ r_req = neg_value (σ state0)
-       Heq : neg_value (σ r_req) = σ state0
-       Hunstable : σ state0 <> σ r_req
-    *)
-    contradict H.
-    repeat (rewrite_state_equiv; try solve_in_dom).
-    simpl. reduce_eqb.
-    rewrite <- Heq; auto.
-  * (* t = clk_fall_flop_marked *)
-    replace (latch_transition_event l clk_fall σ)
-          with (Event (latch_clk l) Bit0)
-          in Hstep
-          by auto.
-    step_inversion_clean.
-    clear Hin. clear Hdec. Search flop.
-    apply flop_inversion_clk in Hstep3.
-    2:{ solve_all_disjoint. }
-    2:{ apply wf_reset_hidden_1; auto. }
-    2:{ apply wf_hidden_reset_1; auto. }
-    destruct Hstep3 as [Hequiv2 Hclk].
-    combine_state_equiv_on.
-    combine_state_equiv_on_complex; try (simpl; solve_space_set).
-    combine_state_equiv_on_domain.
-    (* Know: H : Bit0 = σ0 clk = Bit1 *)
-    contradict H. rewrite_state_equiv; try solve_in_dom.
-    reduce_eqb; inversion 1.
-  * (* t = clk_fall_state0_marked *)
-    replace (latch_transition_event l clk_fall σ)
-          with (Event (latch_clk l) Bit0)
-          in Hstep
-          by auto.
-    step_inversion_clean.
-    clear Hin. clear Hdec. 
-    apply flop_inversion_clk in Hstep3.
-    2:{ solve_all_disjoint. }
-    2:{ apply wf_reset_hidden_1; auto. }
-    2:{ apply wf_hidden_reset_1; auto. }
-    destruct Hstep3 as [Hequiv2 Hclk].
-    combine_state_equiv_on.
-    combine_state_equiv_on_complex; try (simpl; solve_space_set).
-    combine_state_equiv_on_domain.
-
-    contradict H. rewrite_state_equiv; try solve_in_dom.
-    reduce_eqb; inversion 1.
-
-  * (* t = left_req_clk_rise_marked *)
-    replace (latch_transition_event l clk_rise σ)
-          with (Event (latch_clk l) Bit1)
-          in Hstep
-          by auto.
-    step_inversion_clean.
-    apply flop_inversion_clk in Hstep3.
-    2:{ solve_all_disjoint. }
-    2:{ apply wf_reset_hidden_1; auto. }
-    2:{ apply wf_hidden_reset_1; auto. }
-    destruct Hstep3 as [Hequiv2 Hclk].
-    combine_state_equiv_on.
-    combine_state_equiv_on_complex; try (simpl; solve_space_set).
-    combine_state_equiv_on_domain.
-
-    clear Hin. clear Hdec. 
-
-    contradict H1.
-    rewrite_state_equiv; try solve_in_dom.
-    reduce_eqb; inversion 1.
-  * (* t = right_ack_clk_rise_marked *)
-    replace (latch_transition_event l clk_rise σ)
-          with (Event (latch_clk l) Bit1)
-          in Hstep
-          by auto.
-    step_inversion_clean.
-    apply flop_inversion_clk in Hstep3.
-    2:{ solve_all_disjoint. }
-    2:{ apply wf_reset_hidden_1; auto. }
-    2:{ apply wf_hidden_reset_1; auto. }
-    destruct Hstep3 as [Hequiv2 Hclk].
-    combine_state_equiv_on.
-    combine_state_equiv_on_complex; try (simpl; solve_space_set).
-    combine_state_equiv_on_domain.
-
-    clear Hin. clear Hdec. 
-
-    contradict H1.
-    rewrite_state_equiv; try solve_in_dom.
-    reduce_eqb; inversion 1.
-
-  Unshelve. all: exact (fun _ => true).
-
-  Admitted.
-
-(*** HERE ****)
-
-
-Ltac distinguish_events :=
-  match goal with
-  | [ |- context[ Some (latch_transition_event _ ?t _) <> Some (Event _ _) ] ] =>
-    intros; destruct t; auto; inversion 1; fail
-  | [ |- context[ None <> Some _ ] ] => intros; inversion 1
-  | [ |- context[ Some _ <> None ] ] => intros; inversion 1
-  end.
-
-
-Lemma transition_clk_state0 : forall σ σ' t,
-    latch_stage_with_env l ⊢ σ →{Some (latch_transition_event l t σ)} Some σ' ->
-    σ' (latch_state0 l) = σ (latch_state0 l).
-Proof.
-    intros σ σ' t Hstep.
-    destruct t; try find_contradiction;
-        unfold latch_transition_event, transition_event in Hstep.
-    + step_inversion_clean.
-      combine_state_equiv_on_complex; try (simpl; solve_space_set).
-      rewrite_state_equiv; try solve_in_dom.
-      auto.
-    + step_inversion_clean.
-      rewrite_state_equiv; try solve_in_dom.
-      auto.
-    + step_inversion_clean.
-      rewrite_state_equiv; try solve_in_dom.
-      auto.
-    + step_inversion_clean.
-      rewrite_state_equiv; try solve_in_dom.
-      auto.
-    + step_inversion_clean.
-      combine_state_equiv_on_complex; try (simpl; solve_space_set).
-      rewrite_state_equiv; try solve_in_dom.
-      auto.
-    + step_inversion_clean.
-      combine_state_equiv_on_complex; try (simpl; solve_space_set).
-      rewrite_state_equiv; try solve_in_dom.
-      auto.
-
-Unshelve. all:exact (fun _ => true).
-Qed.
-Lemma transition_clk_old_clk : forall σ σ' t,
-    wf_stage_state l σ ->
-    latch_stage_with_env l ⊢ σ →{Some (latch_transition_event l t σ)} Some σ' ->
-    σ' (latch_old_clk l) = σ (latch_old_clk l).
-Proof.
-    intros σ σ' t Hwf Hstep.
-    destruct t; try find_contradiction;
-        unfold latch_transition_event, transition_event in Hstep.
-    + step_inversion_clean.
-      combine_state_equiv_on_complex; try (simpl; solve_space_set).
-      rewrite_state_equiv; try solve_in_dom.
-      auto.
-    + step_inversion_clean.
-      rewrite_state_equiv; try solve_in_dom.
-      auto.
-    + step_inversion_clean.
-      rewrite_state_equiv; try solve_in_dom.
-      auto.
-    + step_inversion_clean.
-      rewrite_state_equiv; try solve_in_dom.
-      auto.
-    + step_inversion_clean.
-      combine_state_equiv_on_complex; try (simpl; solve_space_set).
-      apply flop_inversion_clk in Hstep3.
-      2:{ solve_all_disjoint. }
-      2:{ auto with wf. }
-      2:{ auto with wf. }
-      destruct Hstep3.
-      combine_state_equiv_on.
-      rewrite_state_equiv; try solve_in_dom.
-      auto.
-    + step_inversion_clean.
-      combine_state_equiv_on_complex; try (simpl; solve_space_set).
-      apply flop_inversion_clk in Hstep3.
-      2:{ solve_all_disjoint. }
-      2:{ auto with wf. }
-      2:{ auto with wf. }
-      destruct Hstep3.
-      combine_state_equiv_on.
-      rewrite_state_equiv; try solve_in_dom.
-      auto.
-
-Unshelve. all:exact (fun _ => true).
-Qed.
-
-Section disjoint_place_marked.
-
-  Variable σ σ' : state name.
-  Variable t : token_transition.
-  Hypothesis Hstep : latch_stage_with_env l ⊢ σ →{Some (latch_transition_event l t σ)} Some σ'.
-  Hypothesis Hwf : wf_stage_state l σ. 
-
-  Definition disjoint_place_marked_lemma {t1 t2} (p : stage_place t1 t2) :=
-    t1 <> t -> t2 <> t ->
-    prop_marked p σ' ->
-    prop_marked p σ.
-
-  Lemma disjoint_place_marked_left_ack_left_req : disjoint_place_marked_lemma left_ack_left_req.
-  Proof.
-    intros Ht1 Ht2 Hmarked.
-    dependent destruction Hmarked.
-    constructor.
-      rewrite_back_wf_scoped; try distinguish_events.
-      rewrite_back_wf_scoped; try distinguish_events.
-      auto.
-    Unshelve. all: auto with wf.
-  Qed.
-
-  Lemma disjoint_place_marked_clk_fall_left_ack : disjoint_place_marked_lemma clk_fall_left_ack.
-  Proof.
-    intros Ht1 Ht2 Hmarked.
-    dependent destruction Hmarked.
-    * compare t clk_rise.
-      { (* if the clk+ event happens, contradiction iwth (σ (latch_clk l) = Bit0) *)
-        contradict H.
-        replace (latch_transition_event l clk_rise σ) with (Event (latch_clk l) Bit1) in Hstep
-          by auto.
-        erewrite (wf_update _ (latch_stage_well_formed l) _ _ _ _ Hstep).
-        inversion 1.
-      }
-
-      assert (Hclk : σ0 (latch_clk l) = σ (latch_clk l)).
-      { rewrite_back_wf_scoped; try distinguish_events.
-        auto.
-      }
-
-      assert (Hack : σ0 (ack (latch_input l)) = σ (ack (latch_input l))).
-      { rewrite_back_wf_scoped; try distinguish_events.
-        auto.
-      }
-
-      compare (σ (latch_clk l)) (σ (latch_old_clk l)).
-      2:{ apply clk_fall_left_ack_state0_marked.
-          { rewrite <- Hclk; auto. }
-          { apply val_is_bit_neq in Hneq0; try solve_val_is_bit.
-            rewrite <- Hneq0.
-            rewrite <- Hclk.
-            rewrite H.
-            auto.
-          }
-      }
-      { (* if these are equal, then... *)
-        apply clk_fall_left_ack_marked.
-        { rewrite <- Hclk; auto. }
-        { rewrite <- (transition_clk_state0 σ σ0 t); auto.
-          rewrite <- Hack; auto.
-        }
-      }
-
-    * compare t clk_rise.
-      { (* if the clk+ event happens, contradiction iwth (σ (latch_clk l) = Bit0) *)
-        contradict H.
-        replace (latch_transition_event l clk_rise σ) with (Event (latch_clk l) Bit1) in Hstep
-          by auto.
-        rewrite (wf_update _ (latch_stage_well_formed l) _ _ _ _ Hstep); inversion 1.
-      }
-
-      assert (Hclk : σ0 (latch_clk l) = σ (latch_clk l)).
-      { rewrite_back_wf_scoped; try distinguish_events.
-        auto.
-      }
-
-      apply clk_fall_left_ack_state0_marked.
-      { rewrite <- Hclk; auto. }
-      { erewrite <- transition_clk_old_clk; eauto. }
-
-    Unshelve. all: auto with wf.
-  Qed.
-
-  Lemma disjoint_place_marked_clk_rise_right_req : disjoint_place_marked_lemma clk_rise_right_req.
-  Proof.
-    intros Ht1 Ht2 Hmarked.
-    dependent destruction Hmarked.
-    * assert (Hold_clk : σ (latch_old_clk l) = Bit0).
-      { erewrite <- transition_clk_old_clk; eauto. }
-
-      compare t clk_fall.
-      { unfold latch_transition_event, transition_event in Hstep.
-        step_inversion_clean.
-        decide_events_of Hstep.
-        apply union_inversion_left_only in Hstep; auto.
-        inversion Hstep as [Hstep0 Hequiv0]; clear Hstep.
-        step_inversion_clean. clear Hstep3 Hequiv0.
-        contradict H (* σ0 clk = Bit1 *).
-        rewrite_state_equiv; simpl; try solve_in_dom.
-        reduce_eqb.
-      }
-
-      { assert (Hclk' : σ0 (latch_clk l) = σ (latch_clk l)).
-        { eapply wf_scoped; eauto; try distinguish_events.
-          rewrite latch_stage_with_env_input, latch_stage_with_env_output.
-          solve_space_set.
-        }
-        apply clk_rise_right_req_marked; auto.
-        rewrite <- Hclk'; auto.
-      }
-
-    * apply clk_rise_right_req_marked_state0.
-      intros Heq; contradict H.
-      erewrite transition_clk_state0; eauto.
-
-      erewrite wf_scoped; eauto.
-      2:{ rewrite  latch_stage_with_env_input, latch_stage_with_env_output.
-          solve_space_set.
-      }
-      distinguish_events.
-  Unshelve. exact (fun _ => true).
-  Qed.
-
-  Lemma disjoint_place_marked_right_req_right_ack : disjoint_place_marked_lemma right_req_right_ack.
-  Proof.
-    intros Ht1 Ht2 Hmarked.
-    dependent destruction Hmarked.
-
-    apply rreq_rack_marked.
-    rewrite_back_wf_scoped; try distinguish_events.
-    rewrite_back_wf_scoped; try distinguish_events.
-    auto.
-
-  Unshelve. all:solve_wf.
-  Qed.
-  Lemma disjoint_place_marked_clock_fall : disjoint_place_marked_lemma clock_fall.
-  Proof.
-    Print prop_marked.
-    intros Ht1 Ht2 Hmarked.
-    dependent destruction Hmarked.
-Print prop_marked.
-    * Print token_transition.
-      assert (Hwf' : wf_stage_state l σ0).
-      { eapply step_wf_state_lemma; eauto. }
-      compare t left_req.
-      { unfold latch_transition_event, transition_event in Hstep.
-        step_inversion_clean.
-        decide_events_of Hstep.
-        apply union_inversion_left_only in Hstep; auto.
-        inversion Hstep as [Hstep0 Hequiv0]; clear Hstep.
-        step_inversion_clean.
-        apply func_stable_equiv in H1. 2:{ solve_space_set. }
-
-        (* Since left_req had taken a step, it must have been the case that
-           left_env was unstable in σ.
-           *)
-        assert (Henv : σ (req (latch_input l)) = σ (ack (latch_input l))).
-        { apply neg_value_inj; auto; try solve_val_is_bit. }
-        (* since latch_clk_function l σ0 = Bit1, it must be the case that
-           [latch_clk_function_Bit1_l_req] σ0 (req (latch_input l)) = if_token l (σ0 (latch_state0 l))
-           and thus neg_value (σ (req (latch_input l))) = if_token l (σ state0).
-         *)
-        assert (Hreq : σ (req (latch_input l)) = neg_value (if_token l (σ (latch_state0 l)))).
-        { rewrite H in H1. 
-          symmetry in H1.
-          apply latch_clk_function_Bit1_l_req in H1; auto.
-
-          rewrite <- Hequiv1 in H1; auto.
-          2:{ solve_in_dom. }
-          simpl in H1.
-          unfold update in H1. reduce_eqb.
-          
-          symmetry; apply val_is_bit_neg_inversion; try solve_val_is_bit; symmetry.
-          simpl. rewrite H1.
-          rewrite_state_equiv; try solve_in_dom.
-          simpl.
-          auto.
-        }
-        clear Hin.
-
-
-        assert (Hclk : σ (latch_clk l) = σ0 (latch_clk l)).
-        { rewrite_state_equiv; try solve_in_dom; auto. }
-        assert (Hold_clk : σ (latch_old_clk l) = σ0 (latch_old_clk l)).
-        { rewrite_state_equiv; try solve_in_dom; auto. }
-        compare (latch_clk_function l σ) Bit1.
-        - (* latch_clk_function l σ = Bit1 *)
-          apply clock_fall_flop_marked; auto.
-          { rewrite Hclk; auto. }
-          { rewrite Hold_clk; auto. }
-          { apply func_stable_equiv; try solve_space_set.
-            rewrite Heq0.
-            rewrite Hclk; auto.
-          }
-        - (* latch_clk_function l σ = Bit0 and latch_clk_function l σ0 = Bit1 after changing l_req. *)
-
-          (* Perhaps need to modify prop_marked clock_fall with more information? *)
-          admit.
-    }        
-        
-(*
-      apply func_stable_equiv in H1; try solve_space_set.
-      apply clock_fall_flop_marked; auto.
-      { rewrite_back_wf_scoped; auto. distinguish_events. }
-      { erewrite <- transition_clk_old_clk; eauto. }
-      { apply func_stable_equiv; try solve_space_set.
-        (* need to know latch_clk_function l σ = latch_clk_function l σ0... *)
-        rewrite_back_wf_scoped; auto; try distinguish_events.
-        rewrite (latch_clk_function_equiv σ0); auto.
-        (* We know state0 hasn't changed, and ctrl_reset_n. Waht about l_req and r_ack? *)
-        intros x Hx.
-        decompose_set_structure.
-        { admit (* true *). }
-        { symmetry; eapply transition_clk_state0; eauto. }
-        { compare t 
-rewrite_back_wf_scoped; auto.
-          compare 
-
-      }
-
-clock_fall_flop_marked
-clock_fall_state0_marked
-*)
-
-  Admitted.
-
-
-  Lemma disjoint_place_marked_left_req_clk_rise : disjoint_place_marked_lemma left_req_clk_rise.
-  Admitted.
-
-
-  Lemma disjoint_place_marked_right_ack_clk_rise : disjoint_place_marked_lemma right_ack_clk_rise.
-  Admitted.
-
-End disjoint_place_marked.
-  
-
-  Lemma disjoint_place_marked : forall σ σ' t,
-    latch_stage_with_env l ⊢ σ →{Some (latch_transition_event l t σ)} Some σ' ->
-    wf_stage_state l σ ->
-    forall t1 t2 (p : stage_place t1 t2),
-      t1 <> t ->
-      t2 <> t ->
-      prop_marked p σ' ->
-      prop_marked p σ.
-  Proof.
-    
-    intros σ σ' t Hstep Hwf t1 t2 p Ht1 Ht2 Hmarked.
-    dependent destruction p.
-    * eapply disjoint_place_marked_left_ack_left_req; eauto.
-    * eapply disjoint_place_marked_clk_fall_left_ack; eauto.
-    * eapply disjoint_place_marked_clk_rise_right_req; eauto.
-    * eapply disjoint_place_marked_right_req_right_ack; eauto.
-    * eapply disjoint_place_marked_clock_fall; eauto.
-    * eapply disjoint_place_marked_left_req_clk_rise; eauto.
-    * eapply disjoint_place_marked_right_ack_clk_rise; eauto.
-  Qed.
-    dependent destruction Hmarked.
-    * 
-
-    * constructor.
-      rewrite_back_wf_scoped; try distinguish_events.
-      rewrite_back_wf_scoped; try distinguish_events.
-      auto.
-
-    * 
-
-  * 
-
-    * admit.
-    * admit.
-    * admit.
-    * admit.
-    * admit.
-    * admit.
-
-  Admitted.
-
-  Lemma state_relate_marking_steps : forall σ m,
+  Lemma state_relate_marking_steps : forall l σ m,
     state_relate_marking l σ m ->
     exists tr, latch_stage_with_env l ⊢ σR l →*{tr} Some σ.
   Proof.
-    intros σ m Hrelate.
+    intros l σ m Hrelate.
     induction Hrelate.
     * exists t_empty. constructor.
     * destruct IHHrelate as [tr IH].
@@ -1572,13 +265,13 @@ End disjoint_place_marked.
   Qed.
 
 
-  Lemma relate_implies_marked : forall σ m,
+  Lemma relate_implies_marked : forall l σ m,
     state_relate_marking l σ m ->
     forall {t1 t2} (p : stage_place t1 t2),
-      prop_marked p σ ->
+      prop_marked l p σ ->
       0 < m _ _ p.
   Proof.   (* by induction on state_relate_marking *)
-    intros σ m Hrelate.
+    intros l σ m Hrelate.
     induction Hrelate as [ | ? ? ? ? ? Hrelate IH Hstep Henabled Hm'
                            | ? ? ? Hrelate IH Hstep]; intros t1 t2 p Hp.
     * apply init_relate_implies_marked; auto.
@@ -1586,11 +279,6 @@ End disjoint_place_marked.
       { apply state_relate_marking_steps in Hrelate.
         destruct Hrelate as [tr Hsteps].
         eapply step_wf_state; eauto.
-      }
-      assert (Hwf_stable : wf_stage_state_stable l σ).
-      { apply state_relate_marking_steps in Hrelate.
-        destruct Hrelate as [tr Hsteps].
-        eapply step_wf_state_stable; eauto.
       }
 
       unfold is_enabled in Henabled.
@@ -1600,7 +288,7 @@ End disjoint_place_marked.
       { inversion p; subst; find_contradiction. }
       compare_next.
       { (* t = t2 *) contradict Hp.
-        eapply outgoing_place_not_marked; [ | | eauto]; auto.
+        eapply outgoing_place_not_marked; eauto.
       }
       compare_next.
       { omega. }
@@ -1613,35 +301,29 @@ End disjoint_place_marked.
         destruct Hrelate as [tr Hsteps].
         eapply step_wf_state; eauto.
       }
-      { apply state_relate_marking_steps in Hrelate.
-        destruct Hrelate as [tr Hsteps].
-        eapply step_wf_state_stable; eauto.
-      }
   Qed.
 
-  Theorem state_related_enabled : forall σ σ' t m,
+  Theorem state_related_enabled : forall l σ σ' t m,
     wf_stage_state l σ ->
-    wf_stage_state_stable l σ ->
     latch_stage_with_env l ⊢ σ →{Some (latch_transition_event l t σ)} Some σ' ->
     state_relate_marking l σ m ->
     is_enabled _ t m.
   Proof.
     intros.
     intros t0 p.
-    assert (prop_marked p σ).
+    assert (prop_marked l p σ).
     { eapply step_implies_prop_marked; eauto. }
     eapply relate_implies_marked; eauto.
   Qed.
 
 
-  Lemma step_implies_bit : forall σ x v σ',
+  Lemma step_implies_bit : forall l σ x v σ',
     wf_stage_state l σ ->
-    wf_stage_state_stable l σ ->
 
     latch_stage_with_env l ⊢ σ →{Some (Event x v)} Some σ' ->
     val_is_bit v.
   Proof.
-    intros ? ? ? ? Hwf Hwf_stable Hstep.
+    intros ? ? ? ? ? Hwf Hstep.
     assert (v = σ' x).
     { apply wf_update in Hstep; auto. }
     subst.
@@ -1674,21 +356,17 @@ Ltac solve_bit_neq_neg :=
   end.
 
 
-  Lemma MG_relate_trace_step_lemma :
+  Lemma MG_relate_trace_step_lemma : forall l,
     relate_trace_step_lemma _ (latch_stage_with_env l)
                               (latch_stage_MG_SS l)
         (σR l) (init_stage_MG_state l).
   Proof.
+    intros l.
     unfold relate_trace_step_lemma.
     set (Hdisjoint := scheme_all_disjoint l).
     intros σ1 σ1' σ2 [x v] t Hstep Hrelate.
     assert (Hwfσ1 : wf_stage_state l σ1).
     { eapply step_wf_state.
-      eapply relate_trace_project_left.
-      eauto.
-    }
-    assert (Hwfσ1' : wf_stage_state_stable l σ1).
-    { eapply step_wf_state_stable.
       eapply relate_trace_project_left.
       eauto.
     }
@@ -1706,29 +384,30 @@ Ltac solve_bit_neq_neg :=
       decompose_set_structure.
       + exists left_req; split; [ reflexivity | ].
         simpl.
-        repeat step_inversion_1. rewrite Heq.
-        repeat combine_state_equiv_on. clear Hequiv Hequiv1 Heq0.
+        step_inversion_clean.
+        clear Hin.
         apply val_is_bit_neq in Hunstable; try solve_val_is_bit.
         rewrite val_is_bit_neg_neg in Hunstable; try solve_val_is_bit.
-        rewrite Hunstable; auto.
+        rewrite <- Hunstable; auto.
 
       + exists left_ack; split; [ reflexivity | ].
         simpl.
-        repeat step_inversion_1. 
-        repeat combine_state_equiv_on. clear Hequiv Hequiv1. simpl in Hguard.
+        step_inversion_clean.
+        clear Hin0.
+        combine_state_equiv_on_complex; try (simpl; solve_space_set).
+
         subst.
-        clear Heq.
         symmetry; apply val_is_bit_neq; try solve_val_is_bit.
 
       + exists right_req; split; [ reflexivity | ].
-        repeat step_inversion_1. 
-        repeat combine_state_equiv_on. clear Hequiv Hequiv5. clear Heq.
+        step_inversion_clean.
+
         subst; simpl.
         symmetry; apply val_is_bit_neq; try solve_val_is_bit.
 
       + exists right_ack; split; [ reflexivity | ].
-        repeat step_inversion_1. 
-        repeat combine_state_equiv_on. clear Hequiv Hequiv7. clear Heq0.
+        step_inversion_clean.
+
         subst; simpl.
         symmetry; apply val_is_bit_neq; try solve_val_is_bit.
 
@@ -1746,13 +425,10 @@ Ltac solve_bit_neq_neg :=
     }
     { intros y Hy. reflexivity. }
   Unshelve.
-    exact (fun _ => true).
-    exact (fun _ => true).
-    exact (fun _ => true).
-    exact (fun _ => true).
+    all: exact (fun _ => true).
   Qed.
 
-  Lemma place_name_disjoint_SS : forall t1 t2 (p : place (latch_stage_MG l) t1 t2),
+  Lemma place_name_disjoint_SS : forall l t1 t2 (p : place (latch_stage_MG l) t1 t2),
     place_name (latch_stage_MG l) p ∉ space_domain (latch_stage_with_env l).
   Proof.
     intros.
@@ -1760,9 +436,10 @@ Ltac solve_bit_neq_neg :=
     destruct p; solve_space_set.
   Qed.
 
-  Theorem MG_refines_stage :
+  Theorem MG_refines_stage : forall l,
     traces_of (latch_stage_with_env l) (σR l) ⊆ traces_of (latch_stage_MG_SS l) (init_stage_MG_state l).
   Proof.
+    intros l.
     apply relate_trace_step_subset.
     { intros x Hdom1 Hdom2.
       unfold init_stage_MG_state.
@@ -1775,5 +452,4 @@ Ltac solve_bit_neq_neg :=
   Qed.
 
 
-End prop_marked.
 End ClickMGProofs.
