Click/PropMarked/Outgoing.v
@@ -1,0 +1,324 @@
+
+Require Import Base.
+Require Import Circuit.
+Require Import StateSpace.
+Require Import StateSpace.MarkedGraphs.
+Require Import StateSpace.RelateTrace.
+Require Import Monad.
+
+Require Import List.
+Import ListNotations.
+Open Scope list_scope.
+
+Require Import MarkedGraph.
+Require Import Click.Definitions.
+Require Import Click.Invariants.
+Require Import Click.MG.
+Require Import Click.PropMarked.PropMarked.
+
+
+Import EnsembleNotation.
+Open Scope ensemble_scope.
+Require Import Coq.Program.Equality.
+Require Import Coq.Logic.FunctionalExtensionality.
+
+
+Module OutgoingPlaceNotMarked (Import PropMarked : PropMarkedType).
+  Module PropMarkedTactics := PropMarkedTactics PropMarked.
+  Import PropMarkedTactics.
+  Import PropMarked.ClickMG. (* for stage_place *)
+
+  Lemma outgoing_place_not_marked : forall l σ σ' t,
+    wf_stage_state l σ ->
+    latch_stage_with_env l ⊢ σ →{Some (latch_transition_event l t σ)} Some σ' ->
+    forall t0 (p : stage_place t0 t),
+        ~ prop_marked l p σ'.
+  Proof.
+    intros l σ σ' t Hwf Hstep t0 p Hprop.
+
+    dependent destruction Hprop.
+    * (* t = left_req *)
+      unfold latch_transition_event, transition_event in Hstep.
+
+      step_inversion_clean.
+
+      apply neg_value_inj in Heq; try solve_val_is_bit.
+      (* Know:
+
+         H : σ left_ack = σ0 left_ack = σ0 left_req = neg_value (σ left_req)
+         Heq : σ left_req = σ left_ack
+      *)
+      contradict H.
+      repeat (rewrite_state_equiv; try solve_in_dom).
+      simpl. reduce_eqb.
+      rewrite Heq.
+      apply bit_neq_neg_r; try solve_val_is_bit.
+
+    * (* t = right_ack *)
+      unfold latch_transition_event, transition_event in Hstep.
+      step_inversion_clean.
+
+      (* Know:
+         H : σ right_req = σ0 right_req 
+                         = neg_value (σ0 right_ack)
+                         = neg_value (neg_value (σ right_ack))
+         Heq : neg_value (σ right_ack) = σ right_req
+      *)
+      contradict H.
+      repeat (rewrite_state_equiv; try solve_in_dom).
+      simpl. reduce_eqb.
+      rewrite <- Heq.
+      apply bit_neq_neg_r; solve_val_is_bit.
+
+    * (* t = left_ack (1) *)
+      replace (latch_transition_event l left_ack σ)
+          with (Event (ack (latch_input l)) (neg_value (σ (ack (latch_input l)))))
+          in Hstep
+          by auto.
+      step_inversion_clean.
+      clear Hin0.
+      destruct Hguard as [Hclk Hstate0].
+      combine_state_equiv_on_complex; try (simpl; solve_space_set).
+      (* Know:
+         H : σ clk = σ0 clk = Bit0
+         H0 : neg_value (σ l_ack) = σ0 l_ack = if_token l (σ0 state0) = if_token l (σ state0)
+         Heq : neg_value (σ l_ack) = if_token l (neg_value (σ state0))
+         Hunstable : if_token l (neg_value (σ state0)) <> σ l_ack
+         Hclk : σ clk = Bit0
+         Hstate0 : σ not_state0 = neg_value (σ state0)
+      *)
+      contradict H0.
+      repeat (rewrite_state_equiv; try solve_in_dom).
+      simpl. reduce_eqb.
+      rewrite Heq.
+      destruct l; simpl; [ | apply not_eq_sym ]; apply bit_neq_neg_r; simpl;
+        try solve_val_is_bit.
+
+
+   * (* t = left_ack (2) *)
+
+     replace (latch_transition_event l left_ack σ)
+          with (Event (ack (latch_input l)) (neg_value (σ (ack (latch_input l)))))
+          in Hstep
+          by auto.
+     step_inversion_clean.
+     clear Hin0.
+     combine_state_equiv_on_complex; try (simpl; solve_space_set).
+     destruct Hguard as [Hclk Hstate0].
+     (* Know:
+        H0 : Heq : neg_value l_ack = if_token l (neg_value (σ state0))
+        Hunstable : if_token l (neg_value (σ state0)) <> σ l_ack
+        Hstate0 : σ not_state0 = neg_value (σ state0)
+     *)
+     assert (H_ack_stable : ~ stable (latch_left_ack_component l) σ).
+     { intros [_ Hstable]. (* if it were, then it would not have taken a step *)
+       assert (Hstep' : latch_left_ack_component l ⊢ σ 
+                →{Some (Event (ack (latch_input l)) (neg_value (σ (ack (latch_input l)))))}
+                Some σ0).
+        { apply delay_space_output.
+          3:{ solve_space_set. }
+          3:{ intros x Hx. rewrite_state_equiv; try solve_in_dom.
+              compare_next; auto.
+              decompose_set_structure.
+          }
+          { split; auto. }
+          apply func_output.
+          { simpl. rewrite <- Heq.
+            apply bit_neq_neg_r; try solve_val_is_bit.
+          }
+          { simpl. rewrite <- Heq; auto. }
+          { intros x Hx. rewrite_state_equiv; try solve_in_dom.
+            auto.
+          }
+        }
+        specialize (Hstable _ _ Hstep').
+        inversion Hstable as [? Hstable']; subst.
+        contradict Hstable'.
+        simpl. solve_space_set.
+    }
+
+
+    set (flop_set := match latch_to_token_flag l with
+                     | Token => dp_reset_n
+                     | NonToken => latch_hidden l
+                     end).
+    set (flop_reset := match latch_to_token_flag l with
+                       | NonToken => dp_reset_n
+                       | Token => latch_hidden l
+                     end).
+    assert (H_flop_stable : ~ stable (flop flop_set flop_reset
+                                           (latch_clk l) (latch_old_clk l)
+                                           (latch_not_state0 l) (latch_state0 l))
+                                     σ).
+    { intros Hstable.
+      assert (Hstep : flop flop_set flop_reset
+                           (latch_clk l) (latch_old_clk l)
+                           (latch_not_state0 l) (latch_state0 l)
+                      ⊢ σ →{None} Some (update σ (latch_old_clk l) (σ (latch_clk l)))).
+      { apply Flop_clk_fall; auto.
+        { rewrite Hclk; inversion 1. }
+        { rewrite Hclk.
+          replace (σ (latch_old_clk l)) with (σ0 (latch_old_clk l)).
+          2:{ rewrite_state_equiv; try solve_in_dom. auto. }
+          rewrite H0; inversion 1.
+        }
+        { intros x Hx. auto. }
+       }
+       destruct Hstable as [_ Hstable].
+       specialize (Hstable _ _ Hstep).
+       inversion Hstable.
+    }
+
+
+    (* Know:
+       H : σ clk = σ0 clk = Bit0
+       H0 : σ old_clk = σ0 old_clk = Bit1
+       Heq : neg_value (σ l_ack) = if_token l (neg_value (σ state0))
+         aka σ l_ack = if_token l (σ state0)
+       Hstate0 : σ not_state0 = neg_value (σ state0)
+
+       Heq+wf_left_env ==> σ l_ack <> σ l_req
+    *)
+    (* I think we need to modify the timing constraint/delay so that the clk-
+    event has time to propogate not just to clk, but also to the flop. Can we do
+    this by modifying flop so that clk- events update old_clk automatically??
+    *)
+    admit.
+
+    * (* t = right_req (1) *)
+      replace (latch_transition_event l right_req σ)
+          with (Event (req (latch_output l)) (neg_value (σ (req (latch_output l)))))
+          in Hstep
+          by auto.
+      step_inversion_clean.
+      clear Hin0.
+      (* Know:
+         H : σ clk = σ0 clk = Bit1
+         H0 : σ old_clk = σ0 old_clk = Bit0
+         Heq : neg_value (σ r_req) = σ state0
+         Hunstable : σ state0 <> σ r_req
+      *)
+      (* Since the flop is unstable on clk+, it must be the case that
+         latch_clk_function σ = Bit1 [ BUT WHY?]
+       Therefore, it must be the case that 
+         σ (ack (latch_output l)) = σ (latch_state0 l)
+       from latch_clk_function_Bit1_r_ack.
+       But this means that
+         σ r_ack = neg_value (σ r_req)
+       By wf_right_env, this implies that
+         σ r_req = σ state0
+       which is a contradiction.
+      *)
+      assert (Hfun : latch_clk_function l σ = Bit1).
+      { (* Some invariant about the fact that σ clk = Bit1 and σ old_clk =
+      Bit0.... Or maybe add to prop_marked... *)
+        admit.
+      }
+      apply latch_clk_function_Bit1_r_ack in Hfun; auto.
+      assert (Hunstable' : σ (ack (latch_output l)) = neg_value (σ (req (latch_output l)))).
+      { rewrite Hfun.
+        symmetry in Heq. apply val_is_bit_neg_inversion in Heq; try solve_val_is_bit.
+        simpl. rewrite <- Heq.
+        rewrite val_is_bit_neg_neg; try solve_val_is_bit.
+      }
+      apply wf_right_env in Hunstable'; auto; find_contradiction.
+
+    * (* t = right_req (2) *)
+      replace (latch_transition_event l right_req σ)
+          with (Event (req (latch_output l)) (neg_value (σ (req (latch_output l)))))
+          in Hstep
+          by auto.
+      step_inversion_clean.
+      clear Hin0.
+      (* Know:
+         H : neg_value (σ r_req) = σ0 r_req <> σ0 state0 = σ state0
+         aka    σ r_req = neg_value (σ state0)
+         Heq : neg_value (σ r_req) = σ state0
+         Hunstable : σ state0 <> σ r_req
+      *)
+      contradict H.
+      repeat (rewrite_state_equiv; try solve_in_dom).
+      simpl. reduce_eqb.
+      rewrite <- Heq; auto.
+
+    * (* t = clk_fall_flop_marked *)
+      replace (latch_transition_event l clk_fall σ)
+          with (Event (latch_clk l) Bit0)
+          in Hstep
+          by auto.
+      step_inversion_clean.
+      clear Hin. clear Hdec.
+      apply flop_inversion_clk in Hstep3.
+      2:{ solve_all_disjoint. }
+      2:{ apply wf_reset_hidden_1; auto. }
+      2:{ apply wf_hidden_reset_1; auto. }
+      destruct Hstep3 as [Hequiv2 Hclk].
+      combine_state_equiv_on.
+      combine_state_equiv_on_complex; try (simpl; solve_space_set).
+
+      (* Know: H : Bit0 = σ0 clk = Bit1 *)
+      contradict H. rewrite_state_equiv; try solve_in_dom.
+      reduce_eqb; inversion 1.
+    * (* t = clk_fall_state0_marked *)
+      replace (latch_transition_event l clk_fall σ)
+          with (Event (latch_clk l) Bit0)
+          in Hstep
+          by auto.
+      step_inversion_clean.
+      clear Hin. clear Hdec. 
+      apply flop_inversion_clk in Hstep3.
+      2:{ solve_all_disjoint. }
+      2:{ apply wf_reset_hidden_1; auto. }
+      2:{ apply wf_hidden_reset_1; auto. }
+      destruct Hstep3 as [Hequiv2 Hclk].
+      combine_state_equiv_on.
+      combine_state_equiv_on_complex; try (simpl; solve_space_set).
+
+      contradict H. rewrite_state_equiv; try solve_in_dom.
+      reduce_eqb; inversion 1.
+
+    * (* t = left_req_clk_rise_marked *)
+      replace (latch_transition_event l clk_rise σ)
+          with (Event (latch_clk l) Bit1)
+          in Hstep
+          by auto.
+      step_inversion_clean.
+      apply flop_inversion_clk in Hstep3.
+      2:{ solve_all_disjoint. }
+      2:{ apply wf_reset_hidden_1; auto. }
+      2:{ apply wf_hidden_reset_1; auto. }
+      destruct Hstep3 as [Hequiv2 Hclk].
+      combine_state_equiv_on.
+      combine_state_equiv_on_complex; try (simpl; solve_space_set).
+
+      clear Hin. clear Hdec. 
+
+      contradict H1.
+      rewrite_state_equiv; try solve_in_dom.
+      reduce_eqb; inversion 1.
+
+    * (* t = right_ack_clk_rise_marked *)
+      replace (latch_transition_event l clk_rise σ)
+          with (Event (latch_clk l) Bit1)
+          in Hstep
+          by auto.
+      step_inversion_clean.
+      apply flop_inversion_clk in Hstep3.
+      2:{ solve_all_disjoint. }
+      2:{ apply wf_reset_hidden_1; auto. }
+      2:{ apply wf_hidden_reset_1; auto. }
+      destruct Hstep3 as [Hequiv2 Hclk].
+      combine_state_equiv_on.
+      combine_state_equiv_on_complex; try (simpl; solve_space_set).
+
+      clear Hin. clear Hdec. 
+
+      contradict H1.
+      rewrite_state_equiv; try solve_in_dom.
+      reduce_eqb; inversion 1.
+
+  Unshelve. all: exact (fun _ => true).
+
+  Admitted.
+
+End OutgoingPlaceNotMarked.
