Click/PropMarked/PropMarked.v
@@ -1,0 +1,206 @@
+
+Require Import Base.
+Require Import Circuit.
+Require Import StateSpace.
+Require Import StateSpace.MarkedGraphs.
+Require Import StateSpace.RelateTrace.
+Require Import Monad.
+
+Require Import List.
+Import ListNotations.
+Open Scope list_scope.
+
+Require Import MarkedGraph.
+Require Import Click.Definitions.
+Require Import Click.Invariants.
+Require Import Click.MG.
+
+Require Import Omega.
+
+
+Import EnsembleNotation.
+Open Scope ensemble_scope.
+Require Import Coq.Program.Equality.
+Require Import Coq.Logic.FunctionalExtensionality.
+
+Module Type PropMarkedType.
+  Declare Module ClickModule : ClickType.
+  Export ClickModule.
+  Module ClickMG := ClickMG(ClickModule).
+  Export ClickMG.
+  Export ClickTactics.
+
+  Definition latch_in_flag (l : latch even odd) := swap_token_flag (latch_to_token_flag l).
+  Definition latch_out_flag (l : latch even odd) := latch_to_token_flag l.
+  Definition latch_stage_MG l := stage_MG (latch_in_flag l) (latch_out_flag l).
+  Definition latch_transition_event l := transition_event l (latch_in_flag l).
+  Definition latch_stage_MG_SS l := stage_MG_SS l (latch_in_flag l).
+
+  (** Intuitively, [prop_marked p σ] is a property that holds on a state σ
+  whenever a related marking m satisfies [m(p) > 0]. *)
+
+
+  Inductive prop_marked (l : latch even odd) : forall {t1 t2} (p : stage_place t1 t2) (σ : state name), Prop :=
+
+  (* left_ack -> left_req *)
+  | lack_lreq_marked σ :
+    σ (ack (latch_input l)) = σ (req (latch_input l)) -> prop_marked l left_ack_left_req σ
+
+  (* right_req -> right_ack *)
+  | rreq_rack_marked σ :
+    σ (req (latch_output l)) = neg_value (σ (ack (latch_output l))) ->
+    prop_marked l right_req_right_ack σ (* right_req -> right_ack *)
+
+  (* clk- -> left_ack *)
+  | clk_fall_left_ack_marked σ :
+    σ (latch_clk l) = Bit0 ->
+(*    σ (latch_old_clk l) = Bit0 -> (* i.e. flop component is stable *) *)
+    (* The left_ack component is unstable *)
+    σ (ack (latch_input l)) = match latch_to_token_flag l with
+                              | Token => σ (latch_state0 l)
+                              | Nontoken => neg_value (σ (latch_state0 l))
+                              end ->
+(*    σ (req (latch_input l)) = σ (ack (latch_input l)) -> (* left environment is stable *)*)
+    prop_marked l clk_fall_left_ack σ
+
+  | clk_fall_left_ack_state0_marked σ :
+    σ (latch_clk l) = Bit0 ->
+    σ (latch_old_clk l) = Bit1 ->
+    prop_marked l clk_fall_left_ack σ
+
+  (* clk+ -> right_req *)
+  | clk_rise_right_req_marked σ :
+    σ (latch_clk l) = Bit1 ->
+    σ (latch_old_clk l) = Bit0 ->
+    prop_marked l clk_rise_right_req σ
+  | clk_rise_right_req_marked_state0 σ :
+    σ (req (latch_output l)) <> σ (latch_state0 l) ->
+(*    σ (ack (latch_output l)) <> σ (req (latch_output l)) -> *)
+    prop_marked l clk_rise_right_req σ
+
+  (* clk+ -> clk- *)
+  | clock_fall_flop_marked σ : (* the clk has just risen, and hasn't propogated through the flop yet *)
+    σ (latch_clk l) = Bit1 ->
+    σ (latch_old_clk l) = Bit0 ->
+    stable (latch_clk_component l) σ ->
+    prop_marked l clock_fall σ
+  | clock_fall_state0_marked σ : (* the clk has propogated through the flop, updating state0 *)
+    σ (latch_clk l) = Bit1 ->
+    σ (latch_old_clk l) = Bit1 ->
+    ~ stable (latch_clk_component l) σ ->
+    prop_marked l clock_fall σ
+
+  (* left_req -> clk+ *)
+  | left_req_clk_rise_marked σ :
+    σ (req (latch_input l)) = neg_value (σ (ack (latch_input l))) ->
+    latch_clk_function l σ = Bit1 ->
+    σ (latch_clk l) = Bit0 ->
+    prop_marked l left_req_clk_rise σ
+
+  (* right_ack -> clk+ *)
+  | right_ack_clk_rise_marked σ :
+    σ (ack (latch_output l)) = σ (req (latch_output l)) ->
+    latch_clk_function l σ = Bit1 ->
+    σ (latch_clk l) = Bit0 ->
+    prop_marked l right_ack_clk_rise σ
+  .
+
+End PropMarkedType.
+
+Module PropMarkedTactics (Import PropMarked : PropMarkedType).
+
+  Lemma init_relate_implies_marked : forall {l t1 t2} (p : stage_place t1 t2),
+    prop_marked l p (σR l) ->
+    init_marking (latch_stage_MG l) _ _ p > 0.
+  Proof.
+    intros l t1 t2 p Hp.
+    dependent destruction Hp;
+      try (simpl; unfold init_marking_flag; simpl;
+      unfold σR in *; simpl in *; reduce_eqb;
+      try (destruct l; simpl in *; find_contradiction; auto; fail);
+    fail).
+  Qed.
+
+Lemma wf_reset_hidden_1 : forall l σ,
+    wf_stage_state l σ ->
+    σ match latch_to_token_flag l with
+      | Token => dp_reset_n
+      | NonToken => latch_hidden l
+      end = Bit1.
+Proof.
+  intros ? ? Hwf.
+  destruct l.
+    apply wf_hidden; auto.
+    eapply wf_dp_reset_n; eauto.
+Qed.
+Lemma wf_hidden_reset_1 : forall l σ,
+    wf_stage_state l σ ->
+    σ match latch_to_token_flag l with
+      | Token => latch_hidden l
+      | NonToken => dp_reset_n
+      end = Bit1.
+Proof.
+  intros ? ? Hwf.
+  destruct l.
+    eapply wf_dp_reset_n; eauto.
+    apply wf_hidden; auto.
+Qed.
+Hint Resolve wf_reset_hidden_1 wf_hidden_reset_1 : wf.
+
+(************)
+(** Lemmas **)
+(************)
+
+  Lemma stage_eps_decide_state0 : forall l σ σ0,
+    wf_stage_state l σ ->
+
+    latch_stage_with_env l ⊢ σ →{None} Some σ0 ->
+    σ (latch_state0 l) <> σ0 (latch_state0 l) ->
+    σ (latch_old_clk l) = Bit1 \/ σ (latch_clk l) = Bit1.
+  Proof.
+    intros l σ σ' Hwf Hstep Hstate0.
+    apply step_implies_stage_eps in Hstep; auto.
+    inversion Hstep as [ Hclk Hold_clk Hequiv
+                       | v Hclk Hold_clk Hv Hclk_function Hl_ack Hr_req Hnot_state0 Hequiv
+                       | Hnot_state0 Hclk Hequiv
+                       ]; subst; clear Hstep.
+
+    * left.
+      apply val_is_bit_neq in Hold_clk; try solve_val_is_bit.
+      rewrite <- Hold_clk.
+      apply val_is_bit_neq in Hclk; try solve_val_is_bit.
+
+    * right; auto.
+
+    * contradict Hstate0.
+      rewrite_state_equiv. 2:{ solve_in_dom. }
+      simpl; auto.
+  Qed.
+
+(************)
+(** Tactics *)
+(************)
+
+
+Arguments wf_scoped {name} S {S_wf} σ e σ' Hstep x : rename.
+
+Ltac rewrite_back_wf_scoped :=
+  match goal with
+  | [ Hstep : ?S ⊢ ?σ →{ ?e } Some ?σ' |- context[ ?σ ?x ] ] =>
+    erewrite <- (@wf_scoped _ S _ σ e σ' Hstep x);
+    [ | try (intro; inversion 1; find_contradiction; fail)
+    | rewrite latch_stage_with_env_input, latch_stage_with_env_output;
+          solve_space_set
+    ]
+  end.
+
+
+Ltac distinguish_events :=
+  match goal with
+  | [ |- context[ Some (latch_transition_event _ ?t _) <> Some (Event _ _) ] ] =>
+    intros; destruct t; auto; inversion 1; fail
+  | [ |- context[ None <> Some _ ] ] => intros; inversion 1
+  | [ |- context[ Some _ <> None ] ] => intros; inversion 1
+  end.
+
+End PropMarkedTactics.
