Click/PropMarked/Step.v
@@ -1,0 +1,271 @@
+
+Require Import Base.
+Require Import Circuit.
+Require Import StateSpace.
+Require Import StateSpace.MarkedGraphs.
+Require Import StateSpace.RelateTrace.
+Require Import Monad.
+
+Require Import List.
+Import ListNotations.
+Open Scope list_scope.
+
+Require Import MarkedGraph.
+Require Import Click.Definitions.
+Require Import Click.Invariants.
+Require Import Click.MG.
+Require Import Click.PropMarked.PropMarked.
+
+
+Import EnsembleNotation.
+Open Scope ensemble_scope.
+Require Import Coq.Program.Equality.
+Require Import Coq.Logic.FunctionalExtensionality.
+
+
+Module StepImpliesPropMarked (Import PropMarked : PropMarkedType).
+  Module PropMarkedTactics := PropMarkedTactics PropMarked.
+  Import PropMarkedTactics.
+
+  Section step_implies_prop_marked.
+
+    Variable l : latch even odd.
+    Variable σ σ' : state name.
+    Hypothesis Hwf : wf_stage_state l σ.
+(*    Hypothesis Hwf_stable : wf_stage_state_stable l σ. *)
+
+
+
+  Definition step_implies_prop_marked_spec {t t0} (p : stage_place t0 t) :=
+    latch_stage_with_env l ⊢ σ →{Some (latch_transition_event l t σ)} Some σ' ->
+    prop_marked l p σ.
+
+  Lemma step_implies_prop_marked_left_ack_left_req :
+    step_implies_prop_marked_spec left_ack_left_req.
+  Proof.
+    intros Hstep.
+      constructor.
+      unfold latch_transition_event, transition_event in Hstep.
+      step_inversion_clean.
+
+      apply val_is_bit_neg_inversion in Heq.
+      2:{ solve_val_is_bit. }
+      simpl.
+      rewrite <- Heq.
+      apply val_is_bit_neg_inversion.
+      { solve_val_is_bit. }
+      reflexivity.
+  Unshelve. exact (fun _ => true).
+  Qed.
+
+  Lemma step_implies_prop_marked_clk_fall_left_ack :
+    step_implies_prop_marked_spec clk_fall_left_ack.
+  Proof.
+    intros Hstep. 
+      unfold latch_transition_event, transition_event in Hstep.
+
+      step_inversion_clean.
+      clear Hin0.
+      combine_state_equiv_on_complex.
+      { simpl. solve_space_set. }
+
+      simpl in Hguard. destruct Hguard as [Hclk Hstate0].
+
+      apply clk_fall_left_ack_marked; auto.
+        apply val_is_bit_neq in Hunstable; try solve_val_is_bit.
+        simpl. rewrite <- Hunstable.
+        destruct l; simpl; auto.
+        rewrite val_is_bit_neg_neg; try solve_val_is_bit; auto.
+  Unshelve. exact (fun _ => true).
+  Qed.
+
+  Lemma step_implies_prop_marked_clk_rise_right_req :
+    step_implies_prop_marked_spec clk_rise_right_req.
+  Proof.
+    intros Hstep.
+      replace (latch_transition_event l right_req σ)
+        with  (Event (req (latch_output l)) (neg_value (σ (req (latch_output l)))))
+        in    Hstep
+        by    auto.
+      step_inversion_clean.
+      clear Hin0.
+
+      destruct Hin as [Hin | Hin].
+      2:{ contradict Hin. unfold update. reduce_eqb.
+          apply bit_neq_neg_r; try solve_val_is_bit.
+      }
+      apply clk_rise_right_req_marked_state0.
+      { apply val_is_bit_neq_neg; auto.
+        { right; solve_val_is_bit. }
+      }
+    Unshelve. exact (fun _ => true).
+  Qed. 
+
+  Lemma step_implies_prop_marked_right_req_right_ack :
+    step_implies_prop_marked_spec right_req_right_ack.
+  Proof.
+    intros Hstep.
+      constructor.
+      unfold latch_transition_event, transition_event in Hstep.
+      step_inversion_clean.
+  Unshelve. exact (fun _ => true).
+  Qed.
+
+
+  Lemma step_implies_prop_marked_clock_fall :
+    step_implies_prop_marked_spec clock_fall.
+  Proof.
+    intros Hstep.
+    replace (latch_transition_event l clk_fall σ)
+      with  (Event (latch_clk l) Bit0)
+      in    Hstep
+      by    auto.
+    step_inversion_clean.
+    clear Hin. clear Hdec.
+    combine_state_equiv_on_complex. { simpl; solve_space_set. }
+    
+    apply flop_inversion_clk in Hstep3.
+    2:{ solve_all_disjoint. }
+    2:{ apply wf_reset_hidden_1; auto. }
+    2:{ apply wf_hidden_reset_1; auto. }
+    destruct Hstep3 as [Hequiv' Hstep3].
+    combine_state_equiv_on.
+    standardize_state_equiv_on_set Hequiv0.
+
+    assert (Hclk : σ (latch_clk l) = Bit1).
+    { rewrite <- Heq in *.
+      apply val_is_bit_neq in Hunstable; try solve_val_is_bit.
+    }
+
+    { apply clock_fall_state0_marked; auto.
+      { (* old_clk *) rewrite <- Hstep3; auto. }
+      intros Hstable; apply func_stable_equiv in Hstable.
+      2:{ solve_space_set. }
+      contradict Hstable; auto.
+    }
+
+  Unshelve.
+    exact (fun _ => true).
+  Qed.
+
+  Lemma step_implies_prop_marked_left_req_clk_rise :
+    step_implies_prop_marked_spec left_req_clk_rise.
+  Proof.
+    intros Hstep.
+    replace (latch_transition_event l clk_rise σ)
+      with  (Event (latch_clk l) Bit1)
+      in    Hstep
+      by    auto.
+
+    step_inversion_clean.
+    clear Hin.
+    combine_state_equiv_on_complex. { simpl; solve_space_set. }
+    
+    apply flop_inversion_clk in Hstep3.
+    2:{ solve_all_disjoint. }
+    2:{ apply wf_reset_hidden_1; auto. }
+    2:{ apply wf_hidden_reset_1; auto. }
+
+    destruct Hstep3 as [Hequiv' Hstep3].
+    combine_state_equiv_on.
+
+    apply left_req_clk_rise_marked; auto.
+    { (* Uses latch_clk_function_Bit1_l_req and wf_left_env *)
+      compare (σ (req (latch_input l)))
+              (σ (ack (latch_input l))).
+      2:{ symmetry. apply val_is_bit_neq; try solve_val_is_bit. }
+      symmetry in Heq0.
+      assert (Hreq : σ (req (latch_input l)) <> if_token l (σ (latch_state0 l))).
+      { rewrite <- Heq0. 
+        apply wf_left_env in Heq0; auto.
+        rewrite Heq0.
+        apply not_eq_sym.
+        destruct l; apply bit_neq_neg_r; simpl; solve_val_is_bit.
+      }
+      contradict Hreq.
+      apply latch_clk_function_Bit1_l_req; auto.
+    }
+    { apply val_is_bit_neq in Hunstable;
+        try solve_val_is_bit.
+      2:{ apply latch_clk_function_bit; auto. }
+        simpl. rewrite <- Hunstable.
+        rewrite <- Heq. auto.
+    }
+
+    Unshelve. exact (fun _ => true).
+
+  Qed.
+
+  Lemma step_implies_prop_marked_right_ack_clk_rise :
+    step_implies_prop_marked_spec right_ack_clk_rise.
+  Proof.
+    intros Hstep.
+    replace (latch_transition_event l clk_rise σ)
+      with  (Event (latch_clk l) Bit1)
+      in    Hstep
+      by    auto.
+    step_inversion_clean.
+    clear Hin. clear Hdec.
+    combine_state_equiv_on_complex.
+    { simpl; solve_space_set. }
+
+    apply flop_inversion_clk in Hstep3.
+    2:{ solve_all_disjoint. }
+    2:{ apply wf_reset_hidden_1; auto. }
+    2:{ apply wf_hidden_reset_1; auto. }
+
+    destruct Hstep3 as [Hequiv' Hstep3].
+
+    combine_state_equiv_on.
+
+    apply right_ack_clk_rise_marked; auto.
+    { (* Uses latch_clk_function_Bit1_r_ack and wf_right_env *)
+      compare (σ (req (latch_output l)))
+              (σ (ack (latch_output l))); auto.
+      assert (Hneq1 : σ (req (latch_output l)) = neg_value (σ (ack (latch_output l)))).
+      { symmetry; apply  val_is_bit_neq; try solve_val_is_bit. }
+      assert (Hneq2 : σ (ack (latch_output l)) = neg_value (σ (req (latch_output l)))).
+      { symmetry; apply  val_is_bit_neq; try solve_val_is_bit. }
+      clear Hneq.
+      assert (Hack : σ (ack (latch_output l)) = σ (latch_state0 l)).
+      { apply latch_clk_function_Bit1_r_ack; auto. }
+      apply wf_right_env in Hneq2; auto.
+      contradict Hneq1.
+      { rewrite Hneq2. rewrite Hack.
+        apply bit_neq_neg_r; solve_val_is_bit.
+      }
+    }
+    { rewrite Hstep3.
+      apply val_is_bit_neq in Hunstable; try solve_val_is_bit.
+      2:{ apply latch_clk_function_bit; auto. }
+      rewrite <- Hstep3. simpl.
+      rewrite <- Hunstable.
+      rewrite <- Heq.
+      auto.
+    }
+
+
+    Unshelve. exact (fun _ => true).
+  Qed.
+
+
+  End step_implies_prop_marked.
+
+  Lemma step_implies_prop_marked : forall l σ t σ',
+    wf_stage_state l σ ->
+    latch_stage_with_env l ⊢ σ →{Some (latch_transition_event l t σ)} Some σ' ->
+    forall t0 (p : stage_place t0 t), prop_marked l p σ.
+  Proof.
+    intros l σ t σ' Hwf Hstep t0 p.
+    dependent destruction p.
+    { eapply step_implies_prop_marked_left_ack_left_req; eauto. }
+    { eapply step_implies_prop_marked_clk_fall_left_ack; eauto. }
+    { eapply step_implies_prop_marked_clk_rise_right_req; eauto. }
+    { eapply step_implies_prop_marked_right_req_right_ack; eauto. }
+    { eapply step_implies_prop_marked_clock_fall; eauto. }
+    { eapply step_implies_prop_marked_left_req_clk_rise; eauto. }
+    { eapply step_implies_prop_marked_right_ack_clk_rise; eauto. }
+  Qed.
+
+
+End StepImpliesPropMarked.
