Click/PropMarked/StepPreserved.v
@@ -1,0 +1,747 @@
+
+Require Import Base.
+Require Import Circuit.
+Require Import StateSpace.
+Require Import StateSpace.MarkedGraphs.
+Require Import StateSpace.RelateTrace.
+Require Import Monad.
+
+Require Import List.
+Import ListNotations.
+Open Scope list_scope.
+
+Require Import MarkedGraph.
+Require Import Click.Definitions.
+Require Import Click.Invariants.
+Require Import Click.MG.
+Require Import Click.PropMarked.PropMarked.
+Require Import Click.PropMarked.Step.
+
+
+Import EnsembleNotation.
+Open Scope ensemble_scope.
+Require Import Coq.Program.Equality.
+Require Import Coq.Logic.FunctionalExtensionality.
+
+Module StepPreservation (Import PropMarked : PropMarkedType).
+  Module PropMarkedTactics := PropMarkedTactics PropMarked.
+  Import PropMarkedTactics.
+  Import PropMarked.ClickMG. (* for stage_place *)
+  Module Step := StepImpliesPropMarked PropMarked.
+  Import Step.
+
+
+  (** Lemmas **)
+
+
+  Lemma transition_preserves_state0_old_clk : forall l σ σ' t,
+    wf_stage_state l σ ->
+    latch_stage_with_env l ⊢ σ →{Some (latch_transition_event l t σ)} Some σ' ->
+    σ' (latch_state0 l) = σ (latch_state0 l) /\ σ' (latch_old_clk l) = σ (latch_old_clk l).
+  Proof.
+    intros l σ σ' t Hwf Hstep.
+    destruct t; try find_contradiction;
+        unfold latch_transition_event, transition_event in Hstep.
+    + step_inversion_clean.
+      combine_state_equiv_on_complex; try (simpl; solve_space_set).
+      repeat (rewrite_state_equiv; try solve_in_dom).
+      auto.
+    + step_inversion_clean.
+      repeat (rewrite_state_equiv; try solve_in_dom).
+      auto.
+    + step_inversion_clean.
+      repeat (rewrite_state_equiv; try solve_in_dom).
+      auto.
+    + step_inversion_clean.
+      repeat (rewrite_state_equiv; try solve_in_dom).
+      auto.
+    + step_inversion_clean.
+      combine_state_equiv_on_complex; try (simpl; solve_space_set).
+      apply flop_inversion_clk in Hstep3.
+      2:{ solve_all_disjoint. }
+      2:{ apply wf_reset_hidden_1; auto. }
+      2:{ apply wf_hidden_reset_1; auto. }
+      destruct Hstep3.
+      combine_state_equiv_on.
+      repeat (rewrite_state_equiv; try solve_in_dom).
+      auto.
+    + step_inversion_clean.
+      combine_state_equiv_on_complex; try (simpl; solve_space_set).
+      apply flop_inversion_clk in Hstep3.
+      2:{ solve_all_disjoint. }
+      2:{ apply wf_reset_hidden_1; auto. }
+      2:{ apply wf_hidden_reset_1; auto. }
+      destruct Hstep3.
+      combine_state_equiv_on.
+      repeat (rewrite_state_equiv; try solve_in_dom).
+      auto.
+
+  Unshelve. all:exact (fun _ => true).
+  Qed.
+
+
+  Lemma transition_preserves_state0  : forall l σ σ' t,
+    wf_stage_state l σ ->
+    latch_stage_with_env l ⊢ σ →{Some (latch_transition_event l t σ)} Some σ' ->
+    σ' (latch_state0 l) = σ (latch_state0 l).
+  Proof.
+    intros ? ? ? ? Hwf Hstep.
+    apply transition_preserves_state0_old_clk in Hstep; auto.
+    destruct Hstep; auto.
+  Qed.
+  Lemma transition_preserves_old_clk : forall l σ σ' t,
+    wf_stage_state l σ ->
+    latch_stage_with_env l ⊢ σ →{Some (latch_transition_event l t σ)} Some σ' ->
+    σ' (latch_old_clk l) = σ (latch_old_clk l).
+  Proof.
+    intros ? ? ? ? Hwf Hstep.
+    apply transition_preserves_state0_old_clk in Hstep; auto.
+    destruct Hstep; auto.
+  Qed.
+
+  Lemma latch_clk_function_l_ack_fall : forall l σ σ',
+    wf_stage_state l σ ->
+    wf_stage_state l σ' ->
+    σ (latch_state0 l) = σ' (latch_state0 l) ->
+       σ (ack (latch_output l)) <> σ' (ack (latch_output l))
+    \/ σ (req (latch_input l)) <> σ' (req (latch_input l)) ->
+    latch_clk_function l σ = Bit1 ->
+    latch_clk_function l σ' = Bit0.
+  Proof.
+    intros ? ? ? Hwf Hwf' Hstate0 Hneq Hfun.
+    unfold latch_clk_function, clk_defn, tok_clk_defn in *.
+    erewrite wf_ctrl_reset_n in *; eauto.
+    transitivity (neg_value Bit1); auto.
+    rewrite <- Hstate0; clear Hstate0.
+
+    assert (Hstate0_bit : val_is_bit (σ (latch_state0 l))) by solve_val_is_bit.
+    assert (Hrack_bit : val_is_bit (σ (ack (latch_output l)))) by solve_val_is_bit.
+    assert (Hlreq_bit : val_is_bit (σ (req (latch_input l)))) by solve_val_is_bit.
+    assert (Hrack_bit' : val_is_bit (σ' (ack (latch_output l)))) by solve_val_is_bit.
+    assert (Hlreq_bit' : val_is_bit (σ' (req (latch_input l)))) by solve_val_is_bit.
+    remember (σ (latch_state0 l)) as xstate0.
+    remember (σ (ack (latch_output l))) as xrack.
+    remember (σ (req (latch_input l))) as xlreq.
+    remember (σ' (ack (latch_output l))) as xrack'.
+    remember (σ' (req (latch_input l))) as xlreq'.
+
+        inversion Hstate0_bit as [Hbit | Hbit];
+          rewrite <- Hbit in *; clear xstate0 Hbit Hstate0_bit;
+        inversion Hrack_bit as [Hbit | Hbit];
+          rewrite <- Hbit in *; clear xrack Hbit Hrack_bit;
+        inversion Hlreq_bit as [Hbit | Hbit];
+          rewrite <- Hbit in *; clear xlreq Hbit Hlreq_bit;
+        inversion Hrack_bit' as [Hbit | Hbit];
+          rewrite <- Hbit in *; clear xrack' Hbit Hrack_bit';
+        inversion Hlreq_bit' as [Hbit | Hbit];
+          rewrite <- Hbit in *; clear xlreq' Hbit Hlreq_bit';
+        simpl; simpl in Hfun;
+        try match goal with
+        | [ Hneq : ?x <> ?x \/ ?y <> ?y |- _ ] => destruct Hneq; find_contradiction; fail
+        | [ |- _ ] => destruct l; inversion Hfun; auto; fail
+        end.
+  Qed.
+
+  (********************)
+  (* Non-epsilon step *)
+  (********************)
+
+
+
+Section disjoint_place_marked.
+  Import PropMarkedTactics.
+
+  Variable l : latch even odd.
+  Variable σ σ' : state name.
+  Variable t : token_transition.
+  Hypothesis Hstep : latch_stage_with_env l ⊢ σ →{Some (latch_transition_event l t σ)} Some σ'.
+  Hypothesis Hwf : wf_stage_state l σ. 
+
+  Definition disjoint_place_marked_lemma {t1 t2} (p : stage_place t1 t2) :=
+    t1 <> t -> t2 <> t ->
+    prop_marked l p σ' ->
+    prop_marked l p σ.
+
+  Lemma disjoint_place_marked_left_ack_left_req : disjoint_place_marked_lemma left_ack_left_req.
+  Proof.
+    intros Ht1 Ht2 Hmarked.
+    dependent destruction Hmarked.
+    constructor.
+      rewrite_back_wf_scoped; try distinguish_events.
+      rewrite_back_wf_scoped; try distinguish_events.
+      auto.
+    Unshelve. all: auto with wf.
+  Qed.
+
+  Lemma disjoint_place_marked_clk_fall_left_ack : disjoint_place_marked_lemma clk_fall_left_ack.
+  Proof.
+    intros Ht1 Ht2 Hmarked.
+    dependent destruction Hmarked.
+    * compare t clk_rise.
+      { (* if the clk+ event happens, contradiction iwth (σ (latch_clk l) = Bit0) *)
+        contradict H.
+        replace (latch_transition_event l clk_rise σ) with (Event (latch_clk l) Bit1) in Hstep
+          by auto.
+        erewrite (wf_update _ (latch_stage_well_formed l) _ _ _ _ Hstep).
+        inversion 1.
+      }
+
+      assert (Hclk : σ0 (latch_clk l) = σ (latch_clk l)).
+      { rewrite_back_wf_scoped; try distinguish_events.
+        auto.
+      }
+
+      assert (Hack : σ0 (ack (latch_input l)) = σ (ack (latch_input l))).
+      { rewrite_back_wf_scoped; try distinguish_events.
+        auto.
+      }
+
+      compare (σ (latch_clk l)) (σ (latch_old_clk l)).
+      2:{ apply clk_fall_left_ack_state0_marked.
+          { rewrite <- Hclk; auto. }
+          { apply val_is_bit_neq in Hneq0; try solve_val_is_bit.
+            rewrite <- Hneq0.
+            rewrite <- Hclk.
+            rewrite H.
+            auto.
+          }
+      }
+      { (* if these are equal, then... *)
+        apply clk_fall_left_ack_marked.
+        { rewrite <- Hclk; auto. }
+        { rewrite <- (transition_preserves_state0 l σ σ0 t); auto.
+          rewrite <- Hack; auto.
+        }
+      }
+
+    * compare t clk_rise.
+      { (* if the clk+ event happens, contradiction iwth (σ (latch_clk l) = Bit0) *)
+        contradict H.
+        replace (latch_transition_event l clk_rise σ) with (Event (latch_clk l) Bit1) in Hstep
+          by auto.
+        rewrite (wf_update _ (latch_stage_well_formed l) _ _ _ _ Hstep); inversion 1.
+      }
+
+      assert (Hclk : σ0 (latch_clk l) = σ (latch_clk l)).
+      { rewrite_back_wf_scoped; try distinguish_events.
+        auto.
+      }
+
+      apply clk_fall_left_ack_state0_marked.
+      { rewrite <- Hclk; auto. }
+      { erewrite <- transition_preserves_old_clk; eauto. }
+
+    Unshelve. all: auto with wf.
+  Qed.
+
+  Lemma disjoint_place_marked_clk_rise_right_req : disjoint_place_marked_lemma clk_rise_right_req.
+  Proof.
+    intros Ht1 Ht2 Hmarked.
+    dependent destruction Hmarked.
+    * assert (Hold_clk : σ (latch_old_clk l) = Bit0).
+      { erewrite <- transition_preserves_old_clk; eauto. }
+
+      compare t clk_fall.
+      { unfold latch_transition_event, transition_event in Hstep.
+        step_inversion_clean.
+        decide_events_of Hstep.
+        apply union_inversion_left_only in Hstep; auto.
+        inversion Hstep as [Hstep0 Hequiv0]; clear Hstep.
+        step_inversion_clean. clear Hstep3 Hequiv0.
+        contradict H (* σ0 clk = Bit1 *).
+        rewrite_state_equiv; simpl; try solve_in_dom.
+        reduce_eqb.
+      }
+
+      { assert (Hclk' : σ0 (latch_clk l) = σ (latch_clk l)).
+        { eapply wf_scoped; eauto; try distinguish_events.
+          rewrite latch_stage_with_env_input, latch_stage_with_env_output.
+          solve_space_set.
+        }
+        apply clk_rise_right_req_marked; auto.
+        rewrite <- Hclk'; auto.
+      }
+
+    * apply clk_rise_right_req_marked_state0.
+      intros Heq; contradict H.
+      erewrite transition_preserves_state0; eauto.
+
+      erewrite wf_scoped; eauto.
+      2:{ rewrite  latch_stage_with_env_input, latch_stage_with_env_output.
+          solve_space_set.
+      }
+      distinguish_events.
+  Unshelve. exact (fun _ => true).
+  Qed.
+
+  Lemma disjoint_place_marked_right_req_right_ack : disjoint_place_marked_lemma right_req_right_ack.
+  Proof.
+    intros Ht1 Ht2 Hmarked.
+    dependent destruction Hmarked.
+
+    apply rreq_rack_marked.
+    rewrite_back_wf_scoped; try distinguish_events.
+    rewrite_back_wf_scoped; try distinguish_events.
+    auto.
+
+  Unshelve. all:solve_wf.
+  Qed.
+
+  Lemma disjoint_place_marked_clock_fall : disjoint_place_marked_lemma clock_fall.
+  Proof.
+    intros Ht1 Ht2 Hmarked.
+    dependent destruction Hmarked.
+
+    * assert (Hwf' : wf_stage_state l σ0).
+      { eapply step_wf_state_lemma; eauto. }
+      assert (Hclk : σ (latch_clk l) = Bit1).
+      { rewrite_back_wf_scoped; auto; distinguish_events. }
+      assert (Hold_clk : σ (latch_old_clk l) = Bit0).
+      { erewrite <- transition_preserves_old_clk; eauto. }
+      assert (Hstate0 : σ (latch_state0 l) = σ0 (latch_state0 l)).
+      { erewrite <- transition_preserves_state0; eauto. }
+
+      compare t left_req.
+      {
+
+        apply func_stable_equiv in H1 (* latch_clk_component *); try solve_space_set.
+(*        apply func_stable_equiv in Hmarked (* left_env_component *); try solve_space_set.*)
+        assert (Hfun : latch_clk_function l σ0 = Bit1) by congruence.
+
+        unfold latch_transition_event, transition_event in Hstep.
+        step_inversion_clean.
+        decide_events_of Hstep.
+        apply union_inversion_left_only in Hstep; auto.
+        inversion Hstep as [Hstep0 Hequiv0]; clear Hstep.
+        step_inversion_clean.
+
+        clear Hin. clear Hunstable (* redundant *).
+
+        assert (Hfun' : latch_clk_function l σ = Bit1).
+        { destruct Hin0 as [Hin0 | Hin0].
+          - rewrite Hin0. auto.
+          - rewrite Hin0.
+            rewrite (latch_clk_function_equiv σ0); auto.
+            intros x Hx. apply Hequiv1.
+            decompose_set_structure; solve_in_dom.
+        }
+
+        apply clock_fall_flop_marked; auto.
+        apply func_stable_equiv; try solve_space_set.
+        congruence.
+      }
+
+      compare t right_ack.
+      { apply func_stable_equiv in H1 (* latch_clk_component *); try solve_space_set.
+
+        unfold latch_transition_event, transition_event in Hstep.
+        step_inversion_clean.
+        destruct Hstep. clear Hstep.
+        step_inversion_clean.
+        clear Hin1. clear Hin. clear Hin2.
+        assert (Hfun : latch_clk_function l σ = Bit1).
+        { destruct Hin0 as [Hin0 | Hin0].
+          - rewrite Hin0. auto.
+          - rewrite Hin0.
+            rewrite (latch_clk_function_equiv σ0); auto.
+            { transitivity (latch_clk_function l σ0); auto.
+              rewrite <- H1 (* latch_clk_function *).
+              auto.
+            }
+            { intros x Hx. apply Hequiv1.
+              decompose_set_structure; solve_in_dom.
+            }
+        }
+        apply clock_fall_flop_marked; auto.
+        { apply func_stable_equiv; try solve_space_set.
+          congruence.
+        }
+      }
+
+      { apply func_stable_equiv in H1; try solve_space_set.
+        assert (Hfun : latch_clk_function l σ = Bit1).
+        { rewrite (latch_clk_function_equiv σ0).
+          2:{ intros x Hx.
+              decompose_set_structure.
+              - replace (global_name "ctrl_reset_n") with ctrl_reset_n; auto.
+                repeat erewrite wf_ctrl_reset_n; eauto.
+              - rewrite_back_wf_scoped; auto; distinguish_events.
+              - rewrite_back_wf_scoped; auto; distinguish_events.
+          }
+          transitivity (latch_clk_function l σ0); auto.
+          rewrite <- H1 (* latch_clk_function *).
+          auto.
+        }
+        apply clock_fall_flop_marked; auto.
+        apply func_stable_equiv; try solve_space_set.
+        rewrite Hfun.
+        rewrite_back_wf_scoped; auto; distinguish_events.
+      }
+
+
+  * assert (Hclk : σ (latch_clk l) = Bit1).
+    { rewrite_back_wf_scoped; auto; distinguish_events. }
+    assert (Hold_clk : σ (latch_old_clk l) = Bit1).
+    { erewrite <- transition_preserves_old_clk; eauto. }
+
+    assert (Hfun : latch_clk_function l σ0 = Bit0).
+    { compare (latch_clk_function l σ0) Bit1.
+      2:{ apply not_eq_sym in Hneq.
+          apply val_is_bit_neq in Hneq; try solve_val_is_bit.
+          { apply latch_clk_function_bit; auto.
+            eapply step_wf_state_lemma; eauto.
+          }
+      }
+      { contradict H1 (* latch_clk_component stable *).
+        apply func_stable_equiv; try solve_space_set.
+        rewrite Heq. auto.
+      }
+    }
+
+    assert (Hlack : σ (req (latch_input l)) = σ (ack (latch_input l)) ->
+                    latch_clk_function l σ = Bit0).
+    { intros Heq.
+      compare (latch_clk_function l σ) Bit1; auto.
+      2:{ apply not_eq_sym in Hneq.
+          apply val_is_bit_neq in Hneq; try solve_val_is_bit.
+          apply latch_clk_function_bit; auto.
+      }
+      { apply latch_clk_function_Bit1_l_req in Heq0; auto.
+        contradict Heq0.
+        rewrite Heq.
+        symmetry in Heq; apply wf_left_env in Heq; auto.
+        rewrite Heq.
+        apply not_eq_sym.
+        destruct l; apply bit_neq_neg_r; simpl; try solve_val_is_bit.
+      }
+    }
+
+    assert (Hrreq : σ (ack (latch_output l)) = neg_value (σ (req (latch_output l))) ->
+                    latch_clk_function l σ = Bit0).
+    { intros Heq.
+      compare (latch_clk_function l σ) Bit1; auto.
+      2:{ apply not_eq_sym in Hneq.
+          apply val_is_bit_neq in Hneq; try solve_val_is_bit.
+          apply latch_clk_function_bit; auto.
+      }
+      { apply latch_clk_function_Bit1_r_ack in Heq0; auto.
+        contradict Heq0.
+        rewrite Heq.
+        apply wf_right_env in Heq; auto.
+        rewrite Heq.
+        apply not_eq_sym.
+        destruct l; apply bit_neq_neg_r; simpl; try solve_val_is_bit.
+      }
+    }
+
+    apply clock_fall_state0_marked; auto.
+    { intros Hstable.
+      apply func_stable_equiv in Hstable; try solve_space_set.
+      rewrite Hclk in Hstable.
+      symmetry in Hstable.
+
+      compare t left_req.
+      { assert (Hprop_marked : prop_marked l left_ack_left_req σ ).
+        { eapply step_implies_prop_marked; eauto. }
+        inversion Hprop_marked;
+          subst; clear Hprop_marked; rename H2 into Hprop_marked.
+        symmetry in Hprop_marked.
+        specialize (Hlack Hprop_marked).
+        find_contradiction.
+      }
+
+      compare t right_ack.
+      { assert (Hprop_marked : prop_marked l right_req_right_ack σ ).
+        { eapply step_implies_prop_marked; eauto. }
+        inversion Hprop_marked;
+          subst; clear Hprop_marked; rename H2 into Hprop_marked.
+        apply val_is_bit_neg_inversion in Hprop_marked; try solve_val_is_bit.
+        symmetry in Hprop_marked.
+        specialize (Hrreq Hprop_marked).
+        find_contradiction.
+      }
+
+      { (* otherwise *)
+        contradict Hfun.
+        rewrite (latch_clk_function_equiv σ).
+        { rewrite Hstable. inversion 1. }
+        { intros x Hx.
+          decompose_set_structure.
+          { (* ctrl_reset_n *)
+            replace (global_name "ctrl_reset_n") with ctrl_reset_n; auto.
+            erewrite wf_ctrl_reset_n; eauto.
+            erewrite wf_ctrl_reset_n; eauto.
+            eapply step_wf_state_lemma; eauto.
+          }
+          { (* state0 *)
+            transitivity (σ0 (latch_state0 l)); auto. 
+            erewrite transition_preserves_state0; eauto.
+          }
+          { rewrite_back_wf_scoped; auto. distinguish_events. }
+          { rewrite_back_wf_scoped; auto. distinguish_events. }
+        }
+      }
+
+  Unshelve.
+    all: try solve_wf.
+    all: exact (fun _ => true).
+      
+(*
+clock_fall_flop_marked
+clock_fall_state0_marked
+*)
+
+  Admitted.
+
+
+  Lemma disjoint_place_marked_left_req_clk_rise : disjoint_place_marked_lemma left_req_clk_rise.
+  Admitted.
+
+
+  Lemma disjoint_place_marked_right_ack_clk_rise : disjoint_place_marked_lemma right_ack_clk_rise.
+  Admitted.
+
+End disjoint_place_marked.
+  
+
+  Lemma disjoint_place_marked : forall l σ σ' t,
+    latch_stage_with_env l ⊢ σ →{Some (latch_transition_event l t σ)} Some σ' ->
+    wf_stage_state l σ ->
+    forall t1 t2 (p : stage_place t1 t2),
+      t1 <> t ->
+      t2 <> t ->
+      prop_marked l p σ' ->
+      prop_marked l p σ.
+  Proof.
+    
+    intros l σ σ' t Hstep Hwf t1 t2 p Ht1 Ht2 Hmarked.
+    dependent destruction p.
+    * eapply disjoint_place_marked_left_ack_left_req; eauto.
+    * eapply disjoint_place_marked_clk_fall_left_ack; eauto.
+    * eapply disjoint_place_marked_clk_rise_right_req; eauto.
+    * eapply disjoint_place_marked_right_req_right_ack; eauto.
+    * eapply disjoint_place_marked_clock_fall; eauto.
+    * eapply disjoint_place_marked_left_req_clk_rise; eauto.
+    * eapply disjoint_place_marked_right_ack_clk_rise; eauto.
+  Qed.
+
+  (****************)
+  (* Epsilon step *)
+  (****************)
+
+  Import PropMarkedTactics.
+
+  (* Helper lemmas for relate_implies_marked below *)
+  Lemma relate_implies_marked_eps : forall l σ σ',
+    wf_stage_state l σ ->
+    latch_stage_with_env l ⊢ σ →{None} Some σ' ->
+    forall {t1 t2} (p : stage_place t1 t2),
+    prop_marked l p σ' ->
+    prop_marked l p σ.
+  Proof.
+    intros l σ σ' Hwf Hstep t1 t2 p Hp.
+    dependent destruction Hp.
+    * (* left_ack_left_req *) 
+      (* Because σ0 left_ack = σ0 left_req, if σ →{None} σ0,
+         then it must be the case that σ is equivalent to σ0 on left_ack and left_req. *)
+      apply lack_lreq_marked.
+      rewrite_back_wf_scoped.
+      rewrite_back_wf_scoped.
+      auto.
+
+    * (* right_req_right_ack *)
+      apply rreq_rack_marked.
+      rewrite_back_wf_scoped.
+      rewrite_back_wf_scoped.
+      auto.
+
+    * (* clk_fall_left_ack *)
+      assert (Hclk : σ (latch_clk l) = Bit0).
+      { rewrite_back_wf_scoped; auto. }
+      assert (Hack : σ (ack (latch_input l)) = σ0 (ack (latch_input l))).
+      { rewrite_back_wf_scoped; auto. }
+
+      assert (Hstate0 : σ (latch_state0 l) = σ0 (latch_state0 l) -> prop_marked l clk_fall_left_ack σ).
+      { intros Hstate0.
+        apply clk_fall_left_ack_marked; auto.
+        rewrite Hack. rewrite Hstate0. auto.
+      }
+      assert (Hold_clk : σ (latch_old_clk l) = Bit1 ->
+                        prop_marked l clk_fall_left_ack σ).
+      { intros Hold_clk.
+        apply clk_fall_left_ack_state0_marked; auto.
+      }
+
+      compare (σ (latch_state0 l)) (σ0 (latch_state0 l)); auto.
+      apply stage_eps_decide_state0 in Hstep; auto.
+      destruct Hstep as [Hstep | Hstep]; auto.
+      { find_contradiction. }
+
+    * (* clk_fall_left_ack *)
+      assert (Hclk : σ (latch_clk l) = Bit0) by (rewrite_back_wf_scoped; auto).
+
+      apply clk_fall_left_ack_state0_marked; auto.
+      apply step_implies_stage_eps in Hstep; auto.
+      inversion Hstep; subst; find_contradiction; clear Hstep.
+      + apply val_is_bit_neq in H2; auto; try solve_val_is_bit.
+        rewrite <- H2. rewrite Hclk. auto.
+      + contradict H0.
+        rewrite <- H3. 2:{ solve_in_dom. }
+        unfold update.
+        rewrite <- H2. rewrite Hclk. simpl. inversion 1.
+
+
+    * assert (Hclk : σ (latch_clk l) = Bit1).
+      { rewrite_back_wf_scoped; auto. }
+      apply clk_rise_right_req_marked; auto.
+
+      apply step_implies_stage_eps in Hstep; auto.
+      inversion Hstep; subst; find_contradiction; clear Hstep.
+      + contradict H0. (* old_clk *)
+        rewrite_state_equiv.
+        2:{ solve_in_dom. }
+        reduce_eqb.
+        rewrite Hclk; inversion 1.
+
+      + contradict H0 (* old_clk *).
+        rewrite_state_equiv.
+        2:{ solve_in_dom. }
+        rewrite <- H2, Hclk. simpl. inversion 1.
+
+    * assert (Hclk : σ (req (latch_output l)) = σ0 (req (latch_output l))).
+      { rewrite_back_wf_scoped; auto. }
+
+      apply step_implies_stage_eps in Hstep; auto.
+      inversion Hstep; subst; find_contradiction; clear Hstep.
+      + apply clk_rise_right_req_marked_state0.
+        contradict H.
+        rewrite_state_equiv. 2:{ solve_in_dom. }
+        rewrite_state_equiv. 2:{ solve_in_dom. }
+        simpl. auto.
+
+      + (* If state0 is getting updated, so σ state0 <> σ0 state0... *)
+        apply clk_rise_right_req_marked; auto.
+        apply not_eq_sym in H1.
+        apply val_is_bit_neq in H1 (* old_clk *); try solve_val_is_bit.
+
+      + apply clk_rise_right_req_marked_state0.
+        contradict H.
+        rewrite_state_equiv. 2:{ solve_in_dom. }
+        rewrite_state_equiv. 2:{ solve_in_dom. }
+        simpl. auto.
+
+
+    * (* clk_fall_flop_marked *)
+      assert (Hwf' : wf_stage_state l σ0).
+      { eapply step_wf_state_eps; eauto. }
+      assert (Hclk : σ (latch_clk l) = Bit1).
+      { rewrite_back_wf_scoped; auto. }
+      apply step_implies_stage_eps in Hstep; auto.
+      inversion Hstep; subst; find_contradiction; clear Hstep.
+      2:{ (* not_state gets updated *)
+          contradict H0 (* old_clk *).
+          rewrite_state_equiv; try solve_in_dom. simpl.
+          simpl in *.
+          rewrite <- H3 (* old_clk *).
+          rewrite Hclk.
+          inversion 1.
+      }
+      { (* state0 gets updated *)
+        contradict H0 (* old_clk *).
+        rewrite_state_equiv; try solve_in_dom.
+        reduce_eqb.
+        rewrite Hclk.
+        inversion 1.
+      }
+
+
+    * (* clock_fall *)
+      assert (Hclk : σ (latch_clk l) = Bit1)
+        by (rewrite_back_wf_scoped; auto).
+
+      apply step_implies_stage_eps in Hstep; auto.
+      inversion Hstep; subst; find_contradiction; clear Hstep.
+      + apply clock_fall_flop_marked; auto.
+        { (* old_clk *)
+          apply not_eq_sym in H3. (* old_clk *)
+          apply val_is_bit_neq in H3 (* latch_old_clk *); try solve_val_is_bit.
+        }
+        { (* stable *)
+          apply func_stable_equiv. { solve_space_set. }
+          auto.
+        }
+
+      + apply clock_fall_state0_marked; auto.
+        { (* old_clk *)
+          rewrite <- H3. auto.
+        }
+        { intros Hstable.
+          apply H1.
+          apply func_stable_equiv in Hstable.
+          2:{ solve_space_set. }
+          apply func_stable_equiv.
+          { solve_space_set. }
+          rewrite_state_equiv. 2:{ solve_in_dom. }
+          simpl.
+          rewrite latch_clk_function_equiv with (σ' := σ).
+          2:{ intros x Hx. rewrite <- H4 (* state_equiv_on *).
+              2:{ decompose_set_structure; solve_in_dom. }
+              unfold update. compare_next; auto.
+              contradict Hx; solve_space_set.
+          }
+          auto.
+        }
+
+    * (* left_req_clk_rise *)
+      assert (Hclk : σ (latch_clk l) = σ0 (latch_clk l)).
+      { rewrite_back_wf_scoped; auto. }
+
+      apply left_req_clk_rise_marked; auto.
+      { rewrite_back_wf_scoped. rewrite_back_wf_scoped.
+        auto.
+      }
+      { rewrite latch_clk_function_equiv with (σ' := σ0); auto.
+        { apply step_implies_stage_eps in Hstep; auto.
+          inversion Hstep; subst; find_contradiction; clear Hstep.
+          + intros x Hx.
+            decompose_set_structure; rewrite_state_equiv; auto; solve_in_dom.
+
+          + contradict Hclk.
+            rewrite H1. (* σ0 clk = Bit0 *)
+            rewrite H2. (* σ clk = Bit1 *)
+            inversion 1.
+
+          + intros x Hx.
+            decompose_set_structure; rewrite_state_equiv; auto; solve_in_dom.
+        }
+      }
+      rewrite Hclk. auto.
+
+    * (* right_ack_clk_rise *)
+      assert (Hclk : σ (latch_clk l) = σ0 (latch_clk l)).
+      { rewrite_back_wf_scoped; auto. }
+
+      apply right_ack_clk_rise_marked.
+      { rewrite_back_wf_scoped. rewrite_back_wf_scoped. auto. }
+      { rewrite latch_clk_function_equiv with (σ' := σ0); auto.
+        { apply step_implies_stage_eps in Hstep; auto.
+          inversion Hstep; subst; find_contradiction; clear Hstep.
+          + intros x Hx.
+            decompose_set_structure; rewrite_state_equiv; auto; solve_in_dom.
+
+          + contradict Hclk.
+            rewrite H1 (* σ0 clk = Bit0 *).
+            rewrite H2 (* σ clk = Bit1 *).
+            inversion 1.
+
+          + intros x Hx.
+            decompose_set_structure; rewrite_state_equiv; auto; solve_in_dom.
+        }
+      }
+      { rewrite Hclk. auto. }
+
+  Unshelve. all:auto.
+
+  Qed.
+
+End StepPreservation.
